\begin{enumerate}
\item Let $\mathsf{T}$ be a linear operator on a vector space
  $\mathsf{V}$ over the field $F$, and let $g(t)$ be a polynomial with
  coefficients form $F$. Prove that if $x$ is an eigenvector of
  $\mathsf{T}$ with corresponding eigenvalue $\lambda$, then
  $g(\mathsf{T})(x)= g(\lambda)(x)$. That is, $x$ is an eigenvector of
  $g(\mathsf{T})$ with corresponding eigenvalue $g(\lambda)$.
\item State and prove the comparable results for matrices.
\item Verify (b) for the matrix $A$ in Exercise 3(a) with a
  polynomial $g(t) 2t^2 -t +1$, eigenvector $x
  = \begin{pmatrix}2\\3\end{pmatrix}$, and corresponding eigenvalue
  $\lambda = 4$.
\end{enumerate}
\begin{enumerate}
\item Suppose $\mathsf{T} \in \mathcal{L}(\mathsf{V})$, $\mathsf{V}$
  is a vector space over $F$.

Let $g(t)$ be a polynomial with coefficients from $F$

Claim: If $x$ is an eigenvector of $\mathsf{T}$ with corresponding
eigenvalue $\lambda$ then $g(\mathsf{T})(x) = g(\lambda)x$

Suppose $g(t)$ is of degree $n$;
\begin{align}
\implies g(t) &= a_nx^n +a_{n-1}x^{n-1} +\dotsb+ a_1x + a_o\\
\implies g(\mathsf{T}) &= a_n\mathsf{T}^n + a_{n-1}\mathsf{T}^{n-1}
+\dotsb + a_1\mathsf{T} +a_0\mathsf{I}_{\mathsf{V}}\\
\implies g(\mathsf{T}) (x)&= a_n\mathsf{T}^n(x) + a_{n-1}\mathsf{T}^{n-1}(x)
+\dotsb + a_1\mathsf{T}(x) +a_0\mathsf{I}_{\mathsf{V}}(x)\\
&=a_n\lambda^nx +a_{n-1}\lambda^{n-1}x +\dotsb +a_1\lambda x+ a_0x
\text{ by 5.1.15.a}\\
&=(a_n\lambda^n +a_{n-1}\lambda^{n-1} +\dotsb +a_1\lambda + a_0)x\\
&=g(\lambda)x
\end{align}
\item Prove that if $x$ is an eigenvector of $A$, with corresponding
  eigenvalue $\lambda$ then $g(A)(x) = g(\lambda)(x)$.

Suppose $A \in \mathsf{M}_{n\times n}(F)$, and Let $g(t) \in
\mathsf{P}_n(F)$ such that g(t) is of degree $n$, and $x$ is an
eigenvector of $A$ corresponding to the eigenvalue $\lambda$
\begin{align}
\implies g(t) &= a_nx^n +a_{n-1}x^{n-1} +\dotsb+ a_1x + a_o\\
\implies g(A) &= a_nA^n + a_{n-1}A^{n-1}
+\dotsb + a_1A +a_0I_n\\
\implies g(A) (x)&= a_nA^n(x) + a_{n-1}A^{n-1}(x)
+\dotsb + a_1A(x) +a_0I_n(x)\\
&=a_n\lambda^nx +a_{n-1}\lambda^{n-1}x +\dotsb +a_1\lambda x+
a_0x\text{ by 5.1.15.b}\\
&=(a_n\lambda^n +a_{n-1}\lambda^{n-1} +\dotsb +a_1\lambda + a_0)x\\
&=g(\lambda)x
\end{align}
\item 
\begin{gather}
A  = \begin{pmatrix}
1 & 2\\
3 & 2\\
\end{pmatrix}\\
A^2 =\begin{pmatrix}
7 & 6\\
9 & 10
\end{pmatrix}\\
g(A) = 2\begin{pmatrix}
7 & 6 \\
9 & 10
\end{pmatrix}
-\begin{pmatrix}
1 & 2 \\
2 & 3
\end{pmatrix}
+
\begin{pmatrix}
1 & 0\\
0 & 1
\end{pmatrix}
\end{gather}
\begin{align}
g(A)\begin{pmatrix}2\\3\end{pmatrix} &= 2\begin{pmatrix}
7 & 6 \\
9 & 10
\end{pmatrix}\begin{pmatrix}2\\3\end{pmatrix}
-\begin{pmatrix}
1 & 2 \\
2 & 3
\end{pmatrix}\begin{pmatrix}2\\3\end{pmatrix}
+
\begin{pmatrix}
1 & 0
0 & 1
\end{pmatrix}\begin{pmatrix}2\\3\end{pmatrix}\\
&=
(2)(16)\begin{pmatrix}2\\3\end{pmatrix} +\begin{pmatrix}2\\3\end{pmatrix}
(-1)(4)\begin{pmatrix}2\\3\end{pmatrix}
+ \begin{pmatrix}2\\3\end{pmatrix}\\
&= \left((2)(4^2)+(-1)(4)+(1)\right)\begin{pmatrix}2\\3\end{pmatrix}\\
&= g(4)\begin{pmatrix}2\\3\end{pmatrix}
\end{align}
\end{enumerate}
