For each linear operator $\mathsf{T}$ on $\mathsf{V}$, find the
egienvalues of $\mathsf{T}$ and an ordered bases $\beta$ of
$\mathsf{V}$ such that $[\mathsf{T}]_\beta$ is a diagonal matrix.
\begin{enumerate}
\setcounter{enumii}{2}
\item $\mathsf{V} = \mathsf{R}^3$ and $\mathsf{T}(a,b,c) =(-4a+
  3b-6c,6a-7b+12c,6a-6b+11c)$
\begin{gather}
\alpha =
\left\{\begin{pmatrix}1\\0\\0\end{pmatrix},\begin{pmatrix}0\\1\\0\end{pmatrix},\begin{pmatrix}0\\0\\1\end{pmatrix}\right\}\\
[\mathsf{T}]_\alpha = \begin{pmatrix}
-4 & 3 & -6\\
6 & -7 & 12\\
6 & 6 & 11
\end{pmatrix}
\end{gather}
\begin{align}
\det{([\mathsf{T}]_\alpha -\lambda I_3)} &= \det{\begin{pmatrix}
-4-\lambda & 3 & -6\\
6 & -7-\lambda & 12\\
6 & -6 & 11-\lambda
  \end{pmatrix}}\\
&=\det{\begin{pmatrix}
-4 -\lambda & 4 & -6 \\
6 & -7-\lambda & 12\\
0 & 1+\lambda & 1+\lambda
  \end{pmatrix}}\\
&= (\lambda+4)(\lambda+7)(\lambda+1)\\
&\qquad {} \qquad -2(\lambda+1)(\lambda+1)(\lambda+4)-18(\lambda+1)\\
&=-\lambda^3+3\lambda+2=0\\
&=-(\lambda+1)(\lambda-2)(\lambda+1) =0
\end{align}
\begin{equation}
\implies \lambda=\left\{2,-1\right\}
\end{equation}
\begin{itemize}
\item For $\lambda =2$
\begin{gather}
[\mathsf{T}]_\alpha v = 0\\
([\mathsf{T}]_\alpha -2I)v=0\\
\left(
\begin{pmatrix}
-4 & 3 & -6\\
6 & -7 & 12\\
6 & -6 & 11
\end{pmatrix}
-
2\begin{pmatrix}
1 & 0  &0\\
0 & 1 & 0\\
0 & 0 & 1
\end{pmatrix}
\right)v=0\\
\begin{pmatrix}
-6 & 3 & -6\\
6 & -9 &12\\
6 & -6 & 9
\end{pmatrix}v=0\\
\begin{pmatrix}
-6 & 3 & -6\\
6 & -9 &12\\
6 & -6 & 9
\end{pmatrix}
\leadsto
\begin{pmatrix}
1 & 0 & \mfrac{1}{2}\\
0 & 1 & -1\\
0 & 0 & 0
\end{pmatrix}
\end{gather}
\begin{align}
x_1 &= -\frac{1}{2}t\\
x_2 &= t\\
x_3 &= t
\end{align}
\begin{equation}
v = \left\{t\begin{pmatrix}-\frac{1}{2}\\1\\1\end{pmatrix}\colon t \in \mathbb{R}\right\}
\end{equation}
\item For $\lambda = -1$
\begin{gather}
[\mathsf{T}_\alpha]v = -v\\
[\mathsf{T}]_\alpha]v = 0\\
\left(
\begin{pmatrix}
-4 & 3 & -6\\
6 & -7 & 12\\
6 & -6 & 11
\end{pmatrix}
+
\begin{pmatrix}
1 & 0 & 0\\
0 & 1 & 0\\
0 & 0 & 1
\end{pmatrix}
\right)v=0\\
\begin{pmatrix}
-3 & 3 & -6\\
6 & -6 & 12\\
6 & -6 & 12
\end{pmatrix}v=0\\
\begin{pmatrix}
-3 & 3 & -6\\
6 & -6 & 12\\
6 & -6 & 12
\end{pmatrix}\leadsto
\begin{pmatrix}
1 & -1 & 2\\
0 & 0 & 0\\
0 & 0 & 0
\end{pmatrix}
\end{gather}
\begin{align}
x_1 &= s-2t\\
x_2 &= s\\
x_3 &= t
\end{align}
\begin{equation}
v=\left\{s\begin{pmatrix}1\\1\\0\end{pmatrix}+t\begin{pmatrix}-2\\0\\1\end{pmatrix}\colon
  s,t\in \mathbb{R}^3\right\}
\end{equation}
\end{itemize}
\begin{equation}
\beta =\left\{\begin{pmatrix}-\frac{1}{2}\\-1\\1\end{pmatrix},\begin{pmatrix}1\\1\\0\end{pmatrix},\begin{pmatrix}-1\\0\\1\end{pmatrix}\right\}
\end{equation}
\begin{gather}
[\mathsf{T}]_\beta = Q^{-1}[\mathsf{T}]_\alpha Q\\
Q = \begin{pmatrix}
\mfrac{-1}{2} & 1 & -2\\
1 & 1 & 0\\
1 & 0 & 1
\end{pmatrix}\\
\begin{gmatrix}[left]
\mfrac{-1}{2} & 1 & -2&\\
1 & 1 & 0&\\
1 & 0 & 1&
\end{gmatrix}
\begin{gmatrix}[right]
1 & 0 & 0\\
0 & 1 & 0\\
0 & 0 & 1
\end{gmatrix}
\leadsto
\begin{gmatrix}[left]
1 & 0 & 0&\\
0 & 1 & 0&\\
0 & 0 & 1&
\end{gmatrix}
\begin{gmatrix}[right]
\mfrac{2}{5} & \mfrac{-2}{5} & \mfrac{4}{5}\\
\mfrac{2}{5} & \mfrac{3}{5} & \mfrac{4}{5}\\
\mfrac{-2}{5} & \mfrac{2}{5} & \mfrac{1}{5}
\end{gmatrix}\\
\implies Q^{-1} =
\begin{pmatrix}
\mfrac{2}{5} & \mfrac{-2}{5} & \mfrac{4}{5}\\
\mfrac{2}{5} & \mfrac{3}{5} & \mfrac{4}{5}\\
\mfrac{-2}{5} & \mfrac{2}{5} & \mfrac{1}{5}
\end{pmatrix}
\end{gather}
\begin{align}
[\mathsf{T}]_\beta &= \begin{pmatrix}
\mfrac{2}{5} & \mfrac{-2}{5} & \mfrac{4}{5}\\
\mfrac{2}{5} & \mfrac{3}{5} & \mfrac{4}{5}\\
\mfrac{-2}{5} & \mfrac{2}{5} & \mfrac{1}{5}
\end{pmatrix}
\begin{pmatrix}
-4 & 3 & -6\\
6 & -7 & 12\\
6 & -6 & 11
\end{pmatrix}
\begin{pmatrix}
\mfrac{-1}{2} & 1 & -2&\\
1 & 1 & 0&\\
1 & 0 & 1&
\end{pmatrix}\\
&= \begin{pmatrix}
2 & 0 & 0\\
0 & -1 & 0\\
0 & 0 & -1
\end{pmatrix}
\end{align}
\setcounter{enumii}{4}
\item $\mathsf{V}=\mathsf{P}_3(\mathbb{R})$ and
  $\mathsf{T}(f(x))=xf^\prime(x)+f(2)x+f(3)$
\begin{gather}
\alpha =
\left\{\begin{pmatrix}1\\0\\0\end{pmatrix},\begin{pmatrix}0\\1\\0\end{pmatrix},\begin{pmatrix}0\\0\\1\end{pmatrix}\right\}\\
[\mathsf{T}]_\alpha = \begin{pmatrix}
1 & 3 & 9\\
1 & 3 & 4\\
0 & 0 & 2
\end{pmatrix}
\end{gather}
\begin{align}
\det{([\mathsf{T}]_\alpha-\lambda I)} &= 0\\
&= \det{\begin{pmatrix}
1 -\lambda & 3 & 9\\
1 & 3-\lambda & 4\\
0 & 0 & 2-\lambda
\end{pmatrix}}\\
&= (1-\lambda)(3-\lambda)(2-\lambda)-6(2-\lambda)\\
&=\lambda(2-\lambda)(\lambda-4)
\end{align}
\begin{equation}
\lambda =\{0,2,4\}
\end{equation}
\begin{itemize}
\item For $\lambda =0$
\begin{gather}
Av = 0v\\
Av = 0\\
\begin{pmatrix}
1 & 3 & 9\\
1 & 3 & 4\\
0 & 0 & 2
\end{pmatrix}
\leadsto
\begin{pmatrix}
1 & 3 & 4\\
0 & 0 & 1\\
0 & 0 & 0
\end{pmatrix}
\end{gather}
\begin{align}
x_1 &=-3t\\
x_2 &= t\\
x_3 &= 0
\end{align}
\begin{equation}
v= \left\{t\begin{pmatrix}-3\\1\\0\end{pmatrix}\colon t \in \mathbb{R}\right\}
\end{equation}
\item For $\lambda = 2$
\begin{gather}
Av = 2v\\
(A-2I) = v\\
\begin{pmatrix}
-1 & 3 & 9\\
1 & 1 & 4\\
0 & 0 & 0
\end{pmatrix}v =0\\
\begin{pmatrix}
-1 & 3 & 9\\
1 & 1 & 4\\
0 & 0 & 0
\end{pmatrix}
\leadsto
\begin{pmatrix}
-1 & 3 & 4\\
0 & 4 & 13\\
0 & 0 & 0
\end{pmatrix}
\end{gather}
\begin{align}
x_1 &= -\frac{39}{4}t +9t\\
x_2 &= -\frac{12}{4}t\\
x_3 &= t
\end{align}
\begin{equation}
v = \left\{t\begin{pmatrix}-3\\-13\\4\end{pmatrix}\colon t \in \mathbb{R}\right\}
\end{equation}
\item For $\lambda = 4$
\begin{gather}
Av =4v\\
(A -4I)= v\\
\begin{pmatrix}
-3 & 3 & 9\\
1 & -1 & 4\\
0 & 0 & -2
\end{pmatrix}v =0\\
\begin{pmatrix}
-3 & 3 & 9\\
1 & -1 & 4\\
0 & 0 & -2
\end{pmatrix}
\leadsto
\begin{pmatrix}
0 & 0 & 21\\
1 & -1 & 4\\
0 & 0 & 2
\end{pmatrix}
\end{gather}
\begin{align}
x_1 &= t\\
x_2 &= t\\
x_3 &= 0
\end{align}
\begin{equation}
v = \left\{t\begin{pmatrix}1\\1\\0\end{pmatrix} \colon t \in \mathbb{R}\right\}
\end{equation}
\end{itemize}
\begin{gather}
\beta=
\left\{\begin{pmatrix}-3\\1\\0\end{pmatrix},\begin{pmatrix}-3\\-12\\4\end{pmatrix},\begin{pmatrix}1\\1\\0\end{pmatrix}\right\}\\
\implies \left\{(-3+x),(-3-13x+4x^2),(1+x)\right\}
\end{gather}
\begin{gather}
Q = \begin{pmatrix}
-3 & -3 & 1\\
1 & -13 & 1\\
0 & 4 & 0
\end{pmatrix}\\
\begin{gmatrix}[left]
-3 & -3 & 1&\\
1 & -13 & 1&\\
0 & 4 & 0&
\end{gmatrix}
\begin{gmatrix}[right]
1 & 0 & 0\\
0 & 1 & 0\\
0 & 0 &1
\end{gmatrix}
\leadsto
\begin{gmatrix}[left]
1 & 0 & 0&\\
0 & 1 & 0&\\
0 & 0 &1&
\end{gmatrix}
\begin{gmatrix}[right]
\mfrac{-1}{4} & \mfrac{1}{4} & \mfrac{5}{8}\\
0 & 0 & \mfrac{1}{4}\\
\mfrac{1}{4} &\mfrac{3}{4} & \mfrac{21}{8}
\end{gmatrix}\\
Q^{-1} = \begin{pmatrix}
\mfrac{-1}{4} & \mfrac{1}{4} & \mfrac{5}{8}\\
0 & 0 & \mfrac{1}{4}\\
\mfrac{1}{4} &\mfrac{3}{4} & \mfrac{21}{8}
\end{pmatrix}
\end{gather}
\begin{align}
[\mathsf{T}]_\beta &= Q^{-1}[\mathsf{T}]_\alpha Q\\
&= \begin{pmatrix}
\mfrac{-1}{4} & \mfrac{1}{4} & \mfrac{5}{8}\\
0 & 0 & \mfrac{1}{4}\\
\mfrac{1}{4} &\mfrac{3}{4} & \mfrac{21}{8}
\end{pmatrix}
\begin{pmatrix}
1 & 3 & 9\\
1 & 3 & 4\\
0 & 0 & 2
\end{pmatrix}
\begin{pmatrix}
- 3& -3 & 1\\
1 & -13 & 1\\
0 & 4 & 0
\end{pmatrix}\\
&= \begin{pmatrix}
0 & 0 & 0\\
0 & 2 & 0\\
0 & 0 & 4
\end{pmatrix}
\end{align}
\setcounter{enumii}{7}
\item $\mathsf{V} = \mathsf{M}_{n\times n}(\mathbb{R})$ and
  $\mathsf{T}\begin{pmatrix} a & b\\ c & d\end{pmatrix}
  = \begin{pmatrix} d & b\\ c & a \end{pmatrix}$
\begin{gather}
\alpha = \left\{\begin{pmatrix} 1 & 0 \\ 0 &
     0\end{pmatrix},\begin{pmatrix} 0 & 1 \\ 0 &
     0\end{pmatrix},\begin{pmatrix} 0 & 0 \\ 1 &
     0\end{pmatrix},\begin{pmatrix} 0 & 0 \\ 0 &
     1\end{pmatrix}\right \}\\
[\mathsf{T}]_\alpha = \begin{pmatrix}
0 & 0 & 0 & 1\\
0 & 1 & 0 & 0\\
0 & 0 & 1 & 0\\
1 & 0 & 0 & 0
\end{pmatrix}\\
\det{([\mathsf{T}]_\alpha-\lambda I)} = \det{\begin{pmatrix}
-\lambda & 0 & 0 & 1\\
0 & 1-\lambda & 0 & 0\\
0 & 0 & 1-\lambda & 0\\
1 & 0 & 0 & -\lambda
  \end{pmatrix}}\\
\begin{pmatrix}
-\lambda & 0 & 0 & 1\\
0 & 1-\lambda & 0 & 0\\
0 & 0 & 1-\lambda & 0\\
1 & 0 & 0 & -\lambda
  \end{pmatrix}
\leadsto
\begin{pmatrix}
1 & 0 & 0 & -\lambda\\
0 & 1-\lambda & 0 & 0\\
0 & 0 & 1-\lambda & 0\\
0 & 0 & 0 &1 -\lambda^2
\end{pmatrix}\\
\det{\begin{pmatrix}
1 & 0 & 0 & -\lambda\\
0 & 1-\lambda & 0 & 0\\
0 & 0 & 1-\lambda & 0\\
0 & 0 & 0 &1 -\lambda^2
\end{pmatrix}} = 0\\
\implies (1-\lambda)^2(1-\lambda^2) =0\\
\implies \lambda = \pm 1
\end{gather}
\begin{itemize}
\item For $\lambda = 1$
\begin{gather}
[\mathsf{T}]_\alpha v = v\\
([\mathsf[T]_\alpha - I)v = 0\\
\begin{pmatrix}
-1 & 0 & 0 & 1\\
0 & 0 & 0 & 0\\
0 & 0 & 0 & 0\\
1 & 0 & 0 & -1
\end{pmatrix}v =0
\end{gather}
\begin{align}
x_1 &= t\\
x_2 &= k\\
x_3 &= s\\
x_4 &= t
\end{align}
\begin{equation}
v = \left\{t\begin{pmatrix}1\\0\\0\\1\end{pmatrix}
  +k\begin{pmatrix}0\\1\\0\\0\end{pmatrix}+s\begin{pmatrix}0\\0\\1\\0\end{pmatrix}\colon
  t,k,s \in \mathbb{R}\right\}
\end{equation}
\item For $\lambda = -1$
\begin{gather}
[\mathsf{T}]_\alpha v = v\\
([\mathsf{T}]_\alpha + I)v = 0\\
\begin{pmatrix}
1 & 0 & 0 & 1\\
0 & 2 & 0 & 0\\
0 & 0 & 2 & 0\\
1 & 0 & 0 & 1
\end{pmatrix}v = 0
\end{gather}
\begin{align}
x_1 &= -t\\
x_2 &= 0 \\
x_3 &= 0\\
x_4 &= t
\end{align}
\begin{equation}
v = \left\{t\begin{pmatrix}-1\\0\\0\\1\end{pmatrix}\colon t \in \mathbb{R}\right\}
\end{equation}
\begin{gather}
  \beta =
  \left\{\begin{pmatrix}1\\0\\0\\1\end{pmatrix},\begin{pmatrix}0\\1\\0\\0\end{pmatrix},\begin{pmatrix}0\\0\\1\\0\end{pmatrix},\begin{pmatrix}-1\\0\\0\\1\end{pmatrix}\right\}
  \\
\implies \left\{\begin{pmatrix}1 & 0\\0
    &1\end{pmatrix},\begin{pmatrix}0 & 1\\0
      &0\end{pmatrix},\begin{pmatrix}0 & 0\\1
        &0\end{pmatrix},\begin{pmatrix}-1 & 0\\0
          &1\end{pmatrix}\right\}
 \end{gather}
\end{itemize}
\begin{gather}
Q = \begin{pmatrix}
1 & 0 & 0 & -1\\
0 & 1 & 0 & 0\\
0 & 0 & 1 & 0\\
1 & 0 & 0 & 1
\end{pmatrix}\\
\begin{gmatrix}[left]
1 & 0 & 0 & -1&\\
0 & 1 & 0 & 0&\\
0 & 0 & 1 & 0&\\
1 & 0 & 0 & 1&
\end{gmatrix}
\begin{gmatrix}
1 & 0 & 0 & 0\\
0 & 1 & 0 & 0\\
0 & 0 & 1 & 0\\
0 & 0 & 0 & 1
\end{gmatrix}
\leadsto
\begin{gmatrix}[left]
1 & 0 & 0 & 0&\\
0 & 1 & 0 & 0&\\
0 & 0 & 1 & 0&\\
0 & 0 & 0 & 1&
\end{gmatrix}
\begin{gmatrix}[right]
\mfrac{1}{2} & 0 & 0 & \mfrac{1}{2}\\
0 & 1 & 0 & 0\\
0 & 0 & 1 & 1\\
\mfrac{-1}{2} & 0 & 0 & \mfrac{1}{2}
\end{gmatrix}\\
\implies Q^{-1} = \begin{pmatrix}
\mfrac{1}{2} & 0 & 0 & \mfrac{1}{2}\\
0 & 1 & 0 & 0\\
0 & 0 & 1 & 1\\
\mfrac{-1}{2} & 0 & 0 & \mfrac{1}{2}
\end{pmatrix}
\end{gather}
\begin{align}
[\mathsf{T}]_\beta &= Q^{-1}[\mathsf{T}]_\alpha Q\\
&= \begin{pmatrix}
1 & 0 & 0 & 0&\\
0 & 1 & 0 & 0&\\
0 & 0 & 1 & 0&\\
0 & 0 & 0 & -1&
\end{pmatrix}
\end{align}
\end{enumerate}
