Let $\mathsf{T}$ be a linear operator on a finite-dimensional vector
space $\mathsf{V}$. We define the {\bf determinant} of $\mathsf{T}$,
denoted $\det{(\mathsf{T})}$, as follows: Choose any ordered basis
$\beta$ for $\mathsf{V}$, and define $\det{(\mathsf{T})}=
\det{([\mathsf{T}]_\beta )}$.
\begin{enumerate}
\item Prove that he preceding definition is independent of the choice
  of an ordered basis for $\mathsf{V}$. That is, prove that if $\beta$
  and $\gamma$ are two ordered bases for $\mathsf{V}$, then $\det{([\mathsf{T}]_\beta)}=\det{([\mathsf{T}]_\gamma)}$.
\item Prove that $\mathsf{T}$ is invertible if and only if
  $\det{\mathsf{T}}\neq 0$.
\item Prove that if $\mathsf{T}$ is invertible, then
  $\det{(\mathsf{T}^{-1})}= [\det{(\mathsf{T})}]^{-1}$.
\item Prove that if $\mathsf{U}$ is also a linear operator on
  $\mathsf{V}$, then $\det{(\mathsf{TU})} = \det{(\mathsf{T})}\cdot\det{(\mathsf{U})}$.
\item Prove that $\det{(\mathsf{T}-\lambda \mathsf{I}_\mathsf{V})} =
    \det{[\mathsf{T}]_\beta -\lambda I)}$ for any scalar $\lambda$ and
      any ordered basis $\beta$ for $\mathsf{V}$.
\end{enumerate}
\begin{enumerate}
\item
Suppose $Q$ is the change of coordinates matrix from $\gamma$ to
$\beta$.
\begin{gather}
Q=[\mathsf{I}_\mathsf{V}]_\gamma^\beta \implies
Q^{-1}=[\mathsf{I}_\mathsf{V}]^\gamma_\beta \\
[\mathsf{I}_\mathsf{V}]_\gamma^\beta
[\mathsf{T}]_\gamma[\mathsf{I}_\mathsf{V}]^\gamma_\beta =
[\mathsf{T}]_\beta\\
\implies \det{([\mathsf{I}_\mathsf{V}]_\gamma^\beta
[\mathsf{T}]_\gamma[\mathsf{I}_\mathsf{V}]^\gamma_\beta)} =
\det{[\mathsf{T}]_\beta}\\
\implies\det{[\mathsf{I}_\mathsf{V}]_\gamma^\beta}
\det{[\mathsf{T}]_\gamma}\det{[\mathsf{I}_\mathsf{V}]^\gamma_\beta}\\
[\mathsf{I}_\mathsf{V}]_\gamma^\beta =
([\mathsf{I}_\mathsf{V}]^\gamma_\beta)^{-1}\\
\det{[\mathsf{I}_\mathsf{V}]_\gamma^\beta}=
\det{([\mathsf{I}_\mathsf{V}]^\gamma_\beta)^{-1}}
\end{gather}
\begin{align}
\implies \det{[\mathsf{I}_\mathsf{V}]_\gamma^\beta}
\det{[\mathsf{T}]_\gamma}\det{[\mathsf{I}_\mathsf{V}]^\gamma_\beta} &=
\det{([\mathsf{I}_\mathsf{V}]^\gamma_\beta)^{-1}}\det{[\mathsf{T}]_\gamma}\det{[\mathsf{I}_\mathsf{V}]^\gamma_\beta}\\
&= \det[\mathsf{T}]_\gamma = \det[\mathsf{T}]_\beta
\end{align}
\item 
($\implies$) 

Suppose $\mathsf{T}$ is invertible\\
Suppose $\beta$ is an ordered basis of $\mathsf{V}$.
\begin{gather}
[\mathsf{I}_\mathsf{V}]_\beta = [\mathsf{T}\cdot\mathsf{T}^{-1}]_\beta
= [\mathsf{T}]_\beta[\mathsf{T}^{-1}]_\beta\\
\implies \det{[\mathsf{I}_\mathsf{V}]_\beta} =
\det{[\mathsf{T}]_\beta}\det{[\mathsf{T}^{-1}]_\beta}\\
\det{[\mathsf{I}_\mathsf{V}]_\beta} =1 \\
\implies \det{[\mathsf{T}]_\beta}\det{[\mathsf{T}^{-1}]_\beta} =1\\
\implies \det{[\mathsf{T}]_\beta} \neq 0\\
\implies \det{\mathsf{T}} \neq 0
\end{gather}
($\Leftarrow$)

Suppose $\det{\mathsf{T}}\neq 0$ 
\begin{gather}
\implies \det[\mathsf{T}]_\beta \neq 0 \quad \text{for some ordered
  basis } \beta \text{ of } \mathsf{V}\\
%\det{[\mathsf{T}]_\beta} \neq  0\\
\implies [\mathsf{T}]_\beta \text{ is invertible, by corollary to Th. 4.7}\\ 
\implies \mathsf{T} \text{ is invertible, by corollary to Th. 2.18}
\end{gather}
\item Suppose $\mathsf{T}$ is invertible and $\beta$ is some ordered
  basis of $\mathsf{V}$.
\begin{align}
\det{\mathsf{I}_\mathsf{V}} &= \det{\mathsf{T}\cdot\mathsf{T}^{-1}}\\
&= \det{[\mathsf{T}\cdot\mathsf{T}^{-1}]_\beta}\\
&= \det{[\mathsf{T}]_\beta[\mathsf{T}^{-1}]_\beta}\\
&= \det{[\mathsf{T}]_\beta}\det{[\mathsf{T}^{-1}]_\beta}\\
&= \det{\mathsf{T}}\det{\mathsf{T}^{-1}}
\end{align}
\begin{gather}
\det{\mathsf{I}_\mathsf{V}} = \det{[\mathsf{I}_\mathsf{V}]_\beta} =
  \det{I_n} =1\\
\implies \det{\mathsf{T}} \det{\mathsf{T}^{-1}} = 1\\
\implies \det{\mathsf{T}^{-1}} = (\det{\mathsf{T}})^{-1}
\end{gather}
\item Suppose $\beta$ is an ordered basis of $\mathsf{V}$.
\begin{align}
\det{\mathsf{TU}} &= \det{[\mathsf{TU}]_\beta}\\
&= \det{[\mathsf{T}]_\beta[\mathsf{U}]_\beta} \text{ by Th. 2.11}\\
&= \det{[\mathsf{T}]_\beta}\det{[\mathsf{U}]_\beta} \text{ by Th. 4.7}\\
&= \det{\mathsf{T}}\det{\mathsf{U}}
\end{align}
\item 
\begin{align}
\det{([\mathsf{T}]_\beta -\lambda I)} &= \det{([\mathsf{T}]_\beta
  -\lambda[\mathsf{I}_\mathsf{V}]_\beta)}\\
&= \det{([\mathsf{T}]_\beta
  -[\lambda\mathsf{I}_\mathsf{V}]_\beta)} \text{ by Th. 2.8.b}\\
&= \det{[\mathsf{T}-\lambda \mathsf{I}_\mathsf{V}]_\beta} \text{ by
  Th. 2.8.a}\\
&= \det{(\mathsf{T}-\lambda \mathsf{I}_\mathsf{V})}
\end{align}
\end{enumerate}
