Use Corollary 1 of the spectral theorem to show that if $\mathsf{T}$
is a normal operator on a complex finite-dimensional inner product
space and $\mathsf{U}$ is a linear operator that commutes with
$\mathsf{T},$ then $\mathsf{U}$ commutes with $\mathsf{T}^*.$

\begin{gather}
\mathsf{T} = \lambda_1\mathsf{T}_1 + \lambda_2\mathsf{T}_2 + \dotsb +
\lambda_k\mathsf{T}_k\\ 
\mathsf{T}^* = g(\mathsf{T}) \text{ for some polynomial } g \because
\mathsf{T} \text{ is normal}
\end{gather}
\begin{align}
\mathsf{T}^* &= g(\lambda_1)\mathsf{T}_1^* + g(\lambda_2)\mathsf{T}^* +
\dotsb + g(\lambda_k)\mathsf{T}_k^*\\
&= g(\lambda_1)\mathsf{T}_1 + g(\lambda_2)\mathsf{T} +
\dotsb + g(\lambda_k)\mathsf{T}_k
\end{align}
Because $\mathsf{U}\mathsf{T}=\mathsf{T}\mathsf{U}$ for each
$\mathsf{T}_i,$ $\mathsf{U}\mathsf{T}_i=\mathsf{T}_i\mathsf{U}$ 
\begin{align}
\implies \mathsf{T}^*\mathsf{U} &= g(\lambda_1)\mathsf{T}_1\mathsf{U}
+ g(\lambda_2)\mathsf{T}\mathsf{U} +
\dotsb + g(\lambda_k)\mathsf{T}_k\mathsf{U}\\
&= g(\lambda_1)\mathsf{U}\mathsf{T}_1
+ g(\lambda_2)\mathsf{U}\mathsf{T} +
\dotsb + g(\lambda_k)\mathsf{U}\mathsf{T}_k\\
&=\mathsf{U}g(\lambda_1)\mathsf{T}_1 + \mathsf{U}g(\lambda_2)\mathsf{T} +
\dotsb +\mathsf{U}g(\lambda_k)\mathsf{T}_k\\
&= \mathsf{U}\mathsf{T}^*
\end{align}
