Let $\mathsf{T}$ be a normal operator on a finite-dimensional complex
inner product space $\mathsf{V}.$ Use the spectral decomposition
$\lambda_1\mathsf{T}_1 + \lambda_2\mathsf{T}_2 + \dotsb +
\lambda_k\mathsf{T}_k$ of $\mathsf{T}$ to prove the following results.
\begin{enumerate}
\item If $g$ is a polynomial, then
\[
g(\mathsf{T}) = \sum\limits_{i=1}^k g(\lambda_i)\mathsf{T}_i
\]
\begin{equation}
g(\mathsf{T}) = a_n\mathsf{T}^n+a_{n-1}\mathsf{T}^{n-1} + \dotsb +
a_1\mathsf{T}
\end{equation}
\begin{multline}
g(\lambda_1\mathsf{T}_1 + \lambda_2\mathsf{T}_2 +\dotsb +
\lambda_k\mathsf{T}_k) = \\
\shoveleft{= a_n(\lambda_1\mathsf{T}_1 + \lambda_2\mathsf{T}_2 +\dotsb +
\lambda_k\mathsf{T}_k)^n +}\\+a_{n+1}(\lambda_1\mathsf{T}_1 + \lambda_2\mathsf{T}_2 +\dotsb+
\lambda_k\mathsf{T}_k)^{n-1} + \dotsb + \\
+ a_1(\lambda_1\mathsf{T}_1 + \lambda_2\mathsf{T}_2 +\dotsb +
\lambda_k\mathsf{T}_k)
\end{multline}
It follows that the cross terms cancel because
$\mathsf{T}_i\mathsf{T}_j = 0$ for $i\neq j$
\begin{multline}
\implies g(\mathsf{T}) = a_n\left(\lambda_1^n\mathsf{T}^n + \lambda_2^n\mathsf{T}_2^n+
\dotsb + \lambda_k^n\mathsf{T}^n_k\right) + \\
+ a_{n-1}\left(\lambda_1^{n-1}\mathsf{T}^{n-1} + \lambda_2^{n-1}\mathsf{T}^{n-1}
+ \dotsb + \lambda^{n-1}_k\mathsf{T}^{n-1}_k\right) + \dotsb +\\
+ a_1\left(\lambda_1\mathsf{T}_1 + \lambda_2\mathsf{T}_2 + \dotsb +
  \lambda_k\mathsf{T}_k\right)
\end{multline}
It follows that $\mathsf{T}^n = \mathsf{T}$ because $\mathsf{T}_i$ is a
projection.
\begin{multline}
\implies g(\mathsf{T}) = a_n\left(\lambda_1^n\mathsf{T} + \lambda_2^n\mathsf{T}_2+
\dotsb + \lambda_k^n\mathsf{T}_k\right) + \\
+ a_{n-1}\left(\lambda_1^{n-1}\mathsf{T} + \lambda_2^{n-1}\mathsf{T}
+ \dotsb + \lambda^{n-1}_k\mathsf{T}_k\right) + \dotsb +\\
+ a_1\left(\lambda_1\mathsf{T}_1 + \lambda_2\mathsf{T}_2 + \dotsb +
  \lambda_k\mathsf{T}_k\right)
\end{multline}
Regroup terms.
\begin{multline}
\implies g(\mathsf{T}) = \left(a_n\lambda_1^n\mathsf{T}_1 +
  a_{n-1}\lambda_1^{n-1}\mathsf{T}_1 + \dotsb +
  \lambda_1\mathsf{T}_1\right) + \\+ \left(a_n\lambda_2^n\mathsf{T}_2 +
  a_{n-1}\lambda_2^{n-1}\mathsf{T}_2 + \dotsb +
  a_1\lambda_2\mathsf{T}_2\right) + \dotsb + \\
+\left(a_n\lambda_k^n\mathsf{T}_k +
  a_{n-1}\lambda_k^{n-1}\mathsf{T}_k + \dotsb +a_1\lambda_k\mathsf{T}_k\right)
\end{multline}
Factoring out each  $\mathsf{T}_i$ yields 
\begin{equation}
g(\mathsf{T}) = \mathsf{T}_1g(\lambda_1) + \mathsf{T}_2g(\lambda_2) +
\dotsb + \mathsf{T}_kg(\lambda_k)
\end{equation}
\item If $\mathsf{T}^n = \mathsf{T}_0$ for some $n,$ then $\mathsf{T}=\mathsf{T}_0$
\begin{align}
\mathsf{T} &= \lambda_1\mathsf{T}_1 + \lambda_2\mathsf{T}_2 + \dotsb +
\lambda_k\mathsf{T}_k\\
\mathsf{T}_0 &= \mathsf{T}^n\\
&= \left(\lambda_1\mathsf{T}_1 + \lambda_2\mathsf{T}_2 + \dotsb +
\lambda_k\mathsf{T}_k\right)^n\\
&= \lambda_1^n\mathsf{T}_1^n + \lambda_2^n\mathsf{T}_2^n + \dotsb +
\lambda_k^n\mathsf{T}_k^n\\
&= \lambda_1^n\mathsf{T}_1 + \lambda_2^n\mathsf{T}_2 + \dotsb + \lambda_k^n\mathsf{T}_k
\end{align}
Let $\lambda_i^n$ be the corresponding eigenvalue of $\mathsf{T}_0.$
All eigenvalues of $\mathsf{T}_0$ must be zero, therefore $\lambda_i^n
= \lambda_i$ 
\begin{align}
\mathsf{T}_0 &= \lambda_1\mathsf{T}_1 + \lambda_2\mathsf{T}_2 + \dotsb
+ \lambda_k\mathsf{T}_k\\
&= \mathsf{T}
\end{align}
\item Let $\mathsf{U}$ be a linear operator on $\mathsf{V}.$ Then
  $\mathsf{U}$ commutes with $\mathsf{T}$ if and only if $\mathsf{U}$
  commutes with each $\mathsf{T}_i.$  

$(\implies)$ Suppose $\mathsf{U}\mathsf{T} = \mathsf{T}\mathsf{U}$.
\begin{gather}
\mathsf{T} = \lambda_1\mathsf{T}_1 + \lambda_2\mathsf{T}_2 + \dotsb +
\lambda_k\mathsf{T}_k\\
\mathsf{U}\mathsf{T} = \lambda_1\mathsf{U}\mathsf{T}_1 +
\lambda_2\mathsf{U}\mathsf{T}_2 + \dotsb +
\lambda_k\mathsf{U}\mathsf{T}_k\\
\mathsf{T}\mathsf{U} = \lambda_1\mathsf{T}_1\mathsf{U} +
\lambda_2\mathsf{T}_2\mathsf{U}  + \dotsb +
\lambda_k\mathsf{T}_k\mathsf{U} \\
\implies  \lambda_1\mathsf{T}_1\mathsf{U} +
\lambda_2\mathsf{T}_2\mathsf{U}  + \dotsb +
\lambda_k\mathsf{T}_k\mathsf{U} = \lambda_1\mathsf{U}\mathsf{T}_1 +
\lambda_2\mathsf{U}\mathsf{T}_2 + \dotsb +
\lambda_k\mathsf{U}\mathsf{T}_k\\
\implies \mathsf{U}\mathsf{T}_i = \mathsf{T}_i\mathsf{U}
\end{gather}

$(\Leftarrow)$ Suppose $\mathsf{U}\mathsf{T}_i = \mathsf{T}_i\mathsf{U}$
\begin{align}
\mathsf{U}\mathsf{T} &= \lambda_1\mathsf{U}\mathsf{T}_i +
\lambda_2\mathsf{U}\mathsf{T}_2 + \dotsb +
\lambda_k\mathsf{U}\mathsf{T}_k\\
&= \lambda_1\mathsf{T}_1\mathsf{U} + \lambda_2\mathsf{T}_2\mathsf{U} +
\dotsb + \lambda_k\mathsf{T}_k\mathsf{U}\\
&= \mathsf{T}\mathsf{U}
\end{align}

\item There exists a nomral operator $\mathsf{U}$ on $\mathsf{V}$ such
  that $\mathsf{U}^2 = \mathsf{T}.$
\begin{align}
\mathsf{T} &= \lambda_1\mathsf{T}_1 + \lambda_2\mathsf{T}_2 + \dotsb +
\lambda_k\mathsf{T}_k\\
&= \lambda_1\mathsf{T}^2_1 + \lambda_2\mathsf{T}_2^2 + \dotsb +
\lambda_k\mathsf{T}_k^2\\
&= \mathsf{U}^2\\
\implies \mathsf{U} &= \sqrt{\lambda_1}\mathsf{T}_1 +
\sqrt{\lambda_2}\mathsf{T}_2 + \dotsb + \sqrt{\lambda_k}\mathsf{T}_k
\end{align}

\item $\mathsf{T}$ is invertible if and only if $\lambda_i \neq 0$ for
  $1 \leq i \leq k$

$(\implies)$ Suppose $\mathsf{T}$ is invertible

\begin{equation}
\mathsf{T} = \lambda_1\mathsf{T}_1 + \lambda_2\mathsf{T}_2 + \dotsb + \lambda_k\mathsf{T}_k
\end{equation}
Let $\mathsf{T}^{-1} = \mathsf{U}$ 
\begin{gather}
\mathsf{U} = \frac{1}{\lambda_1}\mathsf{U}_1 +
\frac{1}{\lambda_2}\mathsf{U}_2 + \dotsb +
\frac{1}{\lambda_k}\mathsf{U}_k\\
\implies \lambda_i \neq 0
\end{gather}

$(\Leftarrow)$ Suppose $\lambda_i \neq 0$
\begin{equation}
\mathsf{T} = \lambda_1\mathsf{T}_1 + \lambda_2\mathsf{T}_2 + \dotsb + \lambda_k\mathsf{T}_k
\end{equation}
$\implies \exists \mathsf{U}$ with eigenvalues
$\frac{1}{\lambda_1},\frac{1}{\lambda_2},\dotsc,\frac{1}{\lambda_k}$ 
\begin{gather}
\mathsf{U} = \frac{1}{\lambda_1}\mathsf{U}_1 +
\frac{1}{\lambda_2}\mathsf{U}_2 + \dotsb +
\frac{1}{\lambda_k}\mathsf{U}_k\\
\mathsf{U}\mathsf{T} =
\frac{\lambda_1}{\lambda_1}\mathsf{U}_1\mathsf{T}_1 + 
\frac{\lambda_2}{\lambda_2}\mathsf{U}_2\mathsf{T}_2 + \dotsb +
\frac{\lambda_k}{\lambda_k}\mathsf{U}_k\mathsf{T}_k\\
\mathsf{U}\mathsf{T} = \mathsf{U}_1\mathsf{T}_1 +
\mathsf{U}_2\mathsf{T}_2 + \dotsb + \mathsf{U}_k\mathsf{T}_k
\end{gather}
Because each $R(\mathsf{T}_i) \subseteq \mathsf{V}$ and each
$\mathsf{U}_i$ is an orthogonal projection each
$\mathsf{U}_i\mathsf{T}_i$ is an orthogonal projection.

Let $\mathsf{S} = \mathsf{U}\mathsf{T}$ with $\mathsf{S}_i =
\mathsf{U}_i\mathsf{T}_i$

\begin{gather}
\mathsf{S} = \mathsf{S}_1 + \mathsf{S}_2 + \dotsb + \mathsf{S}_k\\
\implies \lambda_1 = \lambda_2 = \dotsb = \lambda_k = 1\\
\implies \mathsf{S} = \mathsf{I}_\mathsf{V}\\
\implies \mathsf{U} = \mathsf{T}^{-1}
\end{gather}

\item $\mathsf{T}$ is a projection if and only if every eigenvalue of
  $\mathsf{T}$ is $1$ or $0.$

$(\implies)$ Suppose $\mathsf{T}$ is a projection.

\begin{equation}
\mathsf{T}^n = \mathsf{T}
\end{equation}
\begin{align}
\implies \mathsf{T} &= \left(\lambda_1\mathsf{T}_1 +
  \lambda_2\mathsf{T}_2 + \dotsb + \lambda_k\mathsf{T}\right)^n\\
&= \lambda_1^n\mathsf{T}_1^n + \lambda_2^n\mathsf{T}_2^n + \dotsb +
\lambda_k^n\mathsf{T}_k^n\\
&= \lambda_1^n\mathsf{T}_1 + \lambda_2^n + \dotsb +
\lambda_k^n\mathsf{T}_k
\end{align}
\begin{gather}
\implies \lambda_1^n\mathsf{T}_1 + \lambda_2^n + \dotsb +
\lambda_k^n\mathsf{T}_k = \lambda_1\mathsf{T}_1 +
\lambda_2\mathsf{T}_2 + \dotsb + \lambda_k\mathsf{T}_k\\
\implies \lambda_i^n = \lambda_i \\
\lambda_i^n = \lambda_i  \Leftrightarrow \lambda_i =0 \text{ or } \lambda_i = 1
\end{gather}

$(\Leftarrow)$ Suppose all $\lambda_1 = 0$ or all $\lambda_i = 1$

\paragraph{Case 1:} Suppose all $\lambda_i =1$ 
\begin{align}
\mathsf{T} &= \mathsf{T}_1 + \mathsf{T}_2 + \dotsb + \mathsf{T}_k\\
\mathsf{T}^n &= \left(\mathsf{T}_1 + \mathsf{T}_2 + \dotsb +
  \mathsf{T}_k \right)^n\\ 
&= \mathsf{T}_1^n + \mathsf{T}_2^n + \dotsb + \mathsf{T}_k^n\\
&= \mathsf{T}_1 + \mathsf{T}_2 + \dotsb + \mathsf{T}_k\\
&= \mathsf{T}
\end{align}

\paragraph{Case 1:} Suppose all $\lambda_i =0$ 
\begin{align}
\mathsf{T} &= 0\cdot \mathsf{T}_1 + 0\cdot \mathsf{T}_2 + \dotsb +
0\cdot \mathsf{T}_k\\
&= 0\\
&= 0^n\\
&= \mathsf{T}^n
\end{align}
\item $\mathsf{T}= -\mathsf{T}^*$ if and only if every $\lambda_i$ is
  an imaginary number.

$(\implies)$ Suppose $\mathsf{T}= -\mathsf{T}^*$
\begin{align}
\mathsf{T} &= \lambda_1\mathsf{T}_1 + \lambda_2\mathsf{T}_2 + \dotsb +
\lambda_k\mathsf{T}_k\\ 
\mathsf{T}^* &= \overline{\lambda}_1\mathsf{T}_1^* +
\overline{\lambda}_2\mathsf{T}_2^* + \dotsb +
\overline{\lambda}_k\mathsf{T}_k^*\\ 
&= \overline{\lambda}_1\mathsf{T}_1 +
\overline{\lambda}_2\mathsf{T}_2 + \dotsb +
\overline{\lambda}_k\mathsf{T}_k
\end{align}
\begin{gather}
-\mathsf{T}^* = \mathsf{T}\\
\implies -\overline{\lambda}_1\mathsf{T}_1 -
\overline{\lambda}_2\mathsf{T}_2 - \dotsb -
\overline{\lambda}_k\mathsf{T}_k =  \lambda_1\mathsf{T}_1 +
\lambda_2\mathsf{T}_2 + \dotsb + \lambda_k\mathsf{T}_k\\
\Leftrightarrow -\overline{\lambda}_j = \lambda_j \Leftrightarrow
\lambda_j = c_ji, \quad c \in \mathbb{R}
\end{gather}

$(\Leftarrow)$ Suppose $\lambda_i$ is imaginary.
\begin{align}
\mathsf{T} &= \lambda_1\mathsf{T}_1 + \lambda_2\mathsf{T}_2 + \dotsb +
\lambda_k\mathsf{T}_k\\
\mathsf{T}^* &= \overline{\lambda}_1\mathsf{T}_1^* +
\overline{\lambda}_2\mathsf{T}_2^* + \dotsb + 
\overline{\lambda}_k\mathsf{T}_k^*\\
&= \overline{\lambda}_1\mathsf{T}_1 +
\overline{\lambda}_2\mathsf{T}_2 + \dotsb + 
\overline{\lambda}_k\mathsf{T}_k
\end{align}
\begin{equation}
\lambda_j = c_ji \implies \overline{\lambda}_j = -\lambda_j
\end{equation}
\begin{align}
\mathsf{T}^* &= -\lambda_1\mathsf{T}_1 -\lambda_2\mathsf{T}_2 - \dotsb
- \lambda_k\mathsf{T}_k\\
&= -\mathsf{T}s
\end{align}
\end{enumerate}
