Is there a linear transformation $\mathsf{T}\colon\mathsf{R}^3 \to
\mathsf{R}^2$ such that $\mathsf{T}(1,0,3) = (1,1)$ and
$\mathsf{T}(-2,0,-6) = (2,1)$?
\paragraph{} No since if $\mathsf{T}$ is a linear transformation, by the
defination of a linear transformation $\mathsf{T}(cx) =
c\times\mathsf{T}(x)$. But the given $\mathsf{T}$ shows that
\begin{align}
\mathsf{T}(-2(1,0,3)) = \mathsf{T}(-2,0,-6) = (2,1)\\
-2\mathsf{T}(-2(1,0,3)) = -2 \times (1,1) = (-2,-2)
\end{align}
Since $\mathsf{T}(-2(1,0,3)) \neq -2\mathsf{T}(-2(1,0,3))$ the
transformation $\mathsf{T}$ is not a linear transformation.
