The {\bf classical adjoint} of a $2\times 2$ matrix $A \in
\M{2}{2}{F}$ is the matrix
\begin{equation*}
C = \begin{pmatrix}
A_{22} & - A_{12}\\
-A_{21} & A_{11}
\end{pmatrix}
\end{equation*}
Prove that
\begin{enumerate}
\item $CA = AC = \left[\dete{A}\right]I$
\item $\dete{C} = \dete{A}$
\item The classical adjoint of $A^t$ is $C^t$
\item If $A$ is invertible, then $A^{-1} = \left[\dete{A}\right]^{-1}C$
\end{enumerate}
\begin{enumerate}
\item 
\begin{align}
A & = \begin{pmatrix}A_{11}&A_{12}\\A_{21}&A_{22}\end{pmatrix}\\
C & = \begin{pmatrix}A_{22}&-A_{12}\\-A_{21}&A_{11}\end{pmatrix}
\end{align}
\begin{align}
AC
&= \begin{pmatrix}A_{11}&A_{12}\\A_{21}&A_{22}\end{pmatrix}\begin{pmatrix}A_{22}&-A_{12}\\-A_{21}&A_{11}\end{pmatrix}\\
&= \begin{pmatrix}
A_{11}A_{22} -A_{12}A_{21} &  -A_{12}A_{11} +A_{12}A_{11}\\ 
A_{22}A_{21}-A_{22}A_{21} & -A_{12}A_{21} + A_{11}A_{22}
\end{pmatrix}\\
&= \begin{pmatrix}
A_{11}A_{22} -A_{12}A_{21} &  0\\ 
0 & -A_{12}A_{21} + A_{11}A_{22}
\end{pmatrix}
\end{align}
\begin{align}
CA &= 
\begin{pmatrix}
A_{22} & - A_{12}\\
-A_{21} & A_{11}
\end{pmatrix}
\begin{pmatrix}
A_{11} & A_{12}\\
A_{21} & A_{22}
\end{pmatrix}\\
&= \begin{pmatrix}
A_{22}A_{11}-A_{21}A_{12} & A_{22}A_{12} -A_{12}A_{22} \\
-A_{11}A_{21} + A_{21}A_{11} & -A_{21}A_{11} +A_{11}A_{22}
\end{pmatrix}\\
&= \begin{pmatrix}
A_{11}A_{22} -A_{12}A_{21} &  0\\ 
0 & -A_{12}A_{21} + A_{11}A_{22}
\end{pmatrix}
=AC
\end{align}
\begin{gather}
\dete{A} = A_{11}A_{22} - A_{12}A_{21}\\
\implies AC = CA = \dete{A}I_2
\end{gather}
\item $\dete{C} = A_{22}A_{11} -(-A_{12})(-A_{21}) =
  A_{22}A_{11}-A_{21}A_{12} =\dete{A}$
\item
\begin{align}
A^t &= \begin{pmatrix}
A_{11}  & A_{21}\\
A_{12}  & A_{22}\\
\end{pmatrix}\\
D &= \begin{pmatrix}
A_{22} & -A_{21}\\
-A_{12} & A_{11}
\end{pmatrix}
\end{align}
\paragraph{}It follows that $D$ is the classical adjoint of $A^t$
\begin{equation}
C^t = \begin{pmatrix}
A_{22} & -A_{21}\\
A_{12} & A_{11}
\end{pmatrix} = D
\end{equation}
It follows that $C^t$ is the classical adjoint of $A^t$
\item Suppose $A$ is invertible
\begin{gather}
\implies \exists B \colon AB = BA = I\\
\implies \dete{A} \neq 0 
\end{gather}
\begin{gather}
CA =AC = \dete{A}I\\
\implies [\dete{A}]^{-1}CA  = [\dete{A}]^{-1} = A[\dete{A}]^{-1}C =
I\\
\implies A^{-1} = [\dete{A}]^{-1}C
\end{gather}
\end{enumerate}
