Prove that the determinant of an upper triangular matrix is the
product of its diagonal entries.
\paragraph{}
Suppose $A \in \M{n}{n}{F}$ and $A$ is upper triangular.

Proof by induction.

For $n=1$: $A\in \M{1}{1}{F}\implies \dete{A} = A_{11}$ by definition.

Suppose $\dete{A}$ is the product of its diagonal entries for $1\leq
n\leq k$ 

For $n=k+1$: $A \in \M{k+1}{k+1}{F}$
\begin{gather}
\dete{A} = \sum\limits_{j=1}^{k+1} (-1)^{k+1+j} A_{k+1,j}
\dete{\tilde{A}_{k+1,j}}\\
A_{n+1,j} = 0 \quad \text{for } 1\leq j\leq n\\
\implies \det{A} = (-1)^{(k+1)+(k+1)}
A_{k+1,k+1}\dete{\tilde{A}_{k+1,k+1}}\\
\tilde{A}_{k+1,k+1} = \begin{pmatrix}
a_{11} & a_{12} & \cdots & a_{1,k}\\
     & a_{22} &        & a_{2,k}\\
      &\bigzero& \ddots & \vdots\\
      &&        & a_{k,k}
\end{pmatrix}
\end{gather}
$\tilde{A}_{k+1,k+1} \in \M{n}{n}{F} \implies
\dete{\tilde{A}_{n+1,n+1}}$ is a product of diagonal entries by
induction hypothesis.

\begin{equation}
(-1)^{(n+1)+(n+1)} = (-1)^{2n+2} = (-1)^2(-1)^{2n} = (-1)^{2n}
\end{equation}
\begin{gather}
n \in \mathbb{Z}^+ \implies 2n \text{ is even}\\
\implies (-1)^{2n} = 1\\
\implies \dete{A} = A_{n+1,n+1} \prod\limits_{j=1}^n A_{jj} = \prod\limits_{j=1}^{n+1}A_{jj} 
\end{gather}
