Let $A$ denote the $k\times k$ matrix
\[
\begin{pmatrix}
0 & 0 & \cdots & 0 & -a_0\\
1 & 0 & \cdots & 0 & -a_1\\
0 & 1 & \cdots & 0 & -a_2\\
\vdots& \vdots & & \vdots & \vdots\\
0 & 0 & \cdots & 0 & -a_{k-2}\\
0 & 0 & \cdots & 1 & -a_{k-1}
\end{pmatrix}
\]
where $a_0,a_1,\dotsc,a_{k-1}$ are arbitrary scalars. Prove that the
characteristic polynomial of $A$ is
\[
(-1)^k(a_0 +a_1t + \dotsb + a_{k-1}t^{k-1} + t^k)
\]

Proof by induction on $k.$

Suppose $k=1$
\begin{align}
\implies A &= -a_0\\
\det{(A- tI_1)} &= \det{(-a_0 -t)} \\
&= -a_0 -t \\
&= (-1)^1(a_0 + t^1)
\end{align}

Suppose true for $2 \leq k \leq n-1$

Suppose $k=n$
\begin{gather}
\implies A =
\begin{pmatrix}
0 & 0 & \cdots & 0 & -a_0\\
1 & 0 & \cdots & 0 & -a_1\\
0 & 1 & \cdots & 0 & -a_2\\
\vdots& \vdots & & \vdots & \vdots\\
0 & 0 & \cdots & 0 & -a_{n-2}\\
0 & 0 & \cdots & 1 & -a_{n-1}
\end{pmatrix}\\
\implies A - tI_n =
\begin{pmatrix}
-t & 0 & \cdots & 0 & -a_0\\
1 & -t & \cdots & 0 & -a_1\\
0 & 1 & \cdots & 0 & -a_2\\
\vdots& \vdots & & \vdots & \vdots\\
0 & 0 & \cdots & -t & -a_{n-2}\\
0 & 0 & \cdots & 1 & -a_{n-1} -t
\end{pmatrix}\\
\implies \det{(A-tI_n)} = (-t)(-1)^2\det{\tilde{A}_{11}} +
(a_0)(-1)^{n+1}\det{\tilde{A}_{1n}}
\end{gather}
\begin{align}
\det{\tilde{A}_{11}} &= \det{\begin{pmatrix}
-t & 0 & \cdots & 0 & -a_0\\
1 & -t & \cdots & 0 & -a_1\\
0 & 1 & \cdots & 0 & -a_2\\
\vdots& \vdots & & \vdots & \vdots\\
0 & 0 & \cdots & -t & -a_{n-2}\\
0 & 0 & \cdots & 1 & -a_{n-1} -t
  \end{pmatrix}}\\
&= (-a)^{n-1}(a_1 +a_2 t + \dotsb + a_{n-1}t^{n-2} + t^{n-1}) 
\end{align}
\begin{align}
\det{\tilde{A}_{1n}} &= \det{\begin{pmatrix}
1 & -t & 0 & \cdots & 0 \\
0 & 1 & -t & \cdots & 0  \\
0 & 0 & 1 & \cdots & 0  \\
\vdots & \vdots& \vdots & & \vdots \\
0 & 0 & 0 & \cdots & -t \\
0 & 0 & 0 & \cdots & 1 
    \end{pmatrix}}\\
&= 1 \because (\tilde{A}_{1n})_{ii} =1 \forall i (1\leq i \leq n-1)
\end{align}
\begin{align}
\implies \det{(A-tI_n)} &= (-1)(t)(-1)^{n-1}(a_1 +a_2 t + \dotsb +
a_{n-1}t^{n-2} + t^{n-1}) + (a_0)(-1)^n\\
&= (-1)^n(a_0 + a_1 +a_2 t + \dotsb + a_{n-1}t^{n-2} + t^{n-1})
\end{align}
