In $\mathsf{C}([0,1]),$ let $f(t) = t$ and $g(t) = e^t.$ Compute
$\langle f,g \rangle$ (as defined in Example 3), $\norm{f},\norm{g},$
and $\norm{f+g}.$ Then verify both the Cauchy-Schwartz inequality and
the triangle inequality.
\begin{equation}
\langle f,g \rangle \vcentcolon = \int\limits_0^1 f(t)g(t) \; \mathrm{d}t
\end{equation}
\begin{gather}
\langle f,g\rangle = \int\limits_0^1 te^t \; \mathrm{d}t = 1\\
\norm{f} = \sqrt{\langle f,f \rangle} = \int\limits_0^1 t^2\;
\mathrm{d}t = \frac{1}{\sqrt{3}}\\
\norm{g} = \sqrt{\langle g,g\rangle} = \int\limits_0^1 e^{2t} \;
\mathrm{d}t = \sqrt{\frac{e^2 -1}{2}}\\
\norm{f+g} = \sqrt{\langle f+g,f+g \rangle}
\end{gather}
\begin{align}
\langle f+g,f+g \rangle &= \langle f+g,f\rangle + \langle f+g,g\rangle\\
&=\langle  f,f \rangle + \langle g,f \rangle + \langle f,g \rangle +
\langle g,g\rangle\\
&= \frac{3e^2 + 11}{6}
\end{align}
\begin{equation}
\implies \norm{f+g} = \sqrt{\frac{3e^2 + 11}{6}}
\end{equation}
\paragraph{Cauchy-Schwartz Inequality}
\begin{align}
\norm{f}\norm{g} &\stackrel{?}{\geq} \langle f,g \rangle \\
\sqrt{\frac{3e^2 + 11}{6}} &\stackrel{?}{\geq} 1\\
\implies e^2 &\geq 7 \; \checkmark
\end{align}
\paragraph{Triangle Inequality}
\begin{align}
\norm{f} + \norm{g} &\stackrel{?}{\geq} \norm{f+g}\\
\frac{1}{\sqrt{3}} + \sqrt{\frac{e^2-1}{6}} &\stackrel{?}{\geq}
\sqrt{\frac{3e^2 +11}{6}}\\
\implies \sqrt{\frac{e^2-1}{6}} &\geq 1 \; \checkmark
\end{align}
