Let $\mathsf{V}$ be a finite-dimensional inner product space over $F.$
\begin{enumerate}
\item {\it Pasrseval's Identity.} Let $\{v_1,v_2,\dotsc,v_n\}$ be an
orthonormal basis for $\mathsf{V}.$ For any $x,y \in \mathsf{V}$ prov
that
\[
\langle x,y \rangle = \sum\limits_{i=1}^n \langle x,v_i\rangle
\overline{\langle y,v_i\rangle}
\]
\item Use (a) to prove that if $\beta$ is an orthonormal basis for
  $\mathsf{V}$ with inner product $\langle \cdot, \cdot \rangle,$ then
  for any $x,y \in \mathsf{V}$
\[
\left\langle \phi_\beta(x),\phi_\beta(y)\right\rangle^\prime = \left\langle
[x]_\beta,[y]_\beta\right\rangle^\prime = \left\langle x,y \right\rangle,
\]
where $\langle \cdot,\cdot\rangle^\prime$ is the standard inner
product on $\mathsf{F}^n$.
\end{enumerate}
\begin{enumerate}
\item Suppose $x,y \in \mathsf{V}$
\begin{align}
\implies x = \sum\limits_{i=1}^n a_iv_i & & y = \sum\limits_{i=1}^n b_iv_i
\end{align}
Suppose $\beta$ is an orthonormal basis.
\begin{equation}
\implies \langle v_i,v_j \rangle\; \forall v_i,v_j \in \beta \text{
  such that } i\neq j \; (1\leq i,j \leq n)
\end{equation}
Fix some $k \; (1 \leq k \leq n)$
\begin{align}
\langle x,v_k \rangle &= \left \langle \sum\limits_{i=1}^n
  a_iv_i,v_k\right\rangle \\
&= \sum\limits_{i=1}^n a_i \langle v_i,v_k \rangle\\
&= a_k \langle v_k, v_k \rangle\\
&= a_k \norm{v_k}^2\\
&= a_k
\end{align}
\begin{equation}
\implies \sum\limits_{i=1}^n \langle x,v_i \rangle \overline{\langle
  y,v_i\rangle} = \sum\limits_{i=1}^n a_i\overline{b_i} = \langle x,y\rangle
\end{equation}
\item Suppose $\phi_\beta$ is the coordinate isomorphism from
  $\mathsf{V} \to \mathsf{F}^n$
\begin{equation}
\implies \phi_\beta(x),\phi_\beta(y) \in \mathsf{F}^n
\end{equation}
\begin{align}
\implies \phi_\beta(x) = [x]_\beta
= \begin{pmatrix}a_1\\a_2\\\vdots\\a_n\end{pmatrix} & & \phi_\beta(y)
= [y]_\beta = \begin{pmatrix}b_1\\b_2\\\vdots\\b_n\end{pmatrix}
\end{align}
\begin{gather}
\implies \langle [x]_\beta,[y]_\beta\rangle^\prime =
\sum\limits_{i=1}^n a_i\overline{b_i} = \langle x,y \rangle\\
\therefore \langle \phi_\beta(x) , \phi_\beta(y) \rangle^\prime =
\langle [x]_\beta, [y]_\beta \rangle^\prime = \langle x,y\rangle
\end{gather}
\end{enumerate}
