Let $\mathsf{V}$ be a finite-dimensional vector space, and let
$\mathsf{T}\colon \mathsf{V} \to \mathsf{V}$ be linear.
\begin{enumerate}[(a)]
\item If $\text{rank}(\mathsf{T})=\text{rank}(\mathsf{T}^2)$, prove
  that $\mathsf{R}(\mathsf{T})\cap \mathsf{N}(\mathsf{T}) =
  \{0\}$. Deduce that $\mathsf{V} = \mathsf{R}(\mathsf{T}) \oplus
  \mathsf{N}(\mathsf{T})$
\item Prove that $\mathsf{V} = \mathsf{R}(\mathsf{T}^k) \oplus
  \mathsf{N}(\mathsf{T}^k)$ for some positive integer $k$
\end{enumerate}
\begin{enumerate}[(a)]
\item Suppose $x \in R(\mathsf{T}^2)$
\begin{gather}
\exists a \in \mathsf{V}\;\text{such that } \mathsf{T}(\mathsf{T}(a))
= x\\
\implies x \in R(\mathsf{T})\\
\implies R(\mathsf{T}^2) \subseteq R(\mathsf{T})\\
\text{rank}(\mathsf{T}) = \text{rank}(\mathsf{T}^2)\\
\therefore R(\mathsf{T}) = R(\mathsf{T}^2) \label{one}
\end{gather}
Suppose $x \in N(\mathsf{T})$

\begin{gather}
\implies \mathsf{T}(x) = 0 \\
\implies \mathsf{T}(\mathsf{T}(x)) = 0\\
\implies x \in N(\mathsf{T}^2)
\end{gather}
By dimension theory:
\begin{gather}
\text{dim}(R(\mathsf{T})) + \text{dim}(N(\mathsf{T})) =
\text{dim}(R(\mathsf{T}^2)) + \text{dim}(N(\mathsf{T}^2))\\
\text{dim}(N(\mathsf{T})) = \text{dim}(N(\mathsf{T}^2)) \quad
(\text{by \ref{one}})\\
\implies N(\mathsf{T}) = \mathsf{N}(\mathsf{T}^2) \label{two}
\end{gather}
Claim: $R(\mathsf{T}\cap N(\mathsf{T} = \{0\}$
\\Suppose $u \in R(\mathsf{T}) \cap N(\mathsf{T})$
\begin{gather}
\exists y \in \mathsf{V}\; \text{such that } \mathsf{T}(y) = u\\
\mathsf{T}^2(y) = 0 \\
\therefore y \in N(\mathsf{T}^2)\\
\therefore y \in N(\mathsf{T}) \quad (\text{by \ref{two}})\\
u = \mathsf{T}(y) = 0
\end{gather}
Claim: $V = N(\mathsf{T}) \oplus R(\mathsf{T})$
\\Suppose $\beta_N$ is a basis for $N\mathsf{T}$ and $\beta_R$ is a
basis for $R(\mathsf{T})$
\begin{gather}
N(\mathsf{T}) \cap R(\mathsf{T}) =\{0\}\\
\implies \text{span}(\beta_N)\cap \text{span}(\beta_R)
=\{0\} \label{three}\\
\therefore \beta_N\cap \beta_R = \{\}\\
\implies \text{card}(\beta_N\cup\beta_R) = n\\
\beta_N =\{n_1,n_2,\dotsc,n_k\} \implies \text{card}(\beta_N) = k\\
\beta_R =\{r_1,r_2,\dotsc,r_m\} \implies \text{card}(\beta_R) =m\\
\end{gather}
For $i$ from 1 to $k$ if $n_i \in \text{span}(\beta_R)$
\begin{equation}
\text{span}(\beta_N)\cap\text{span}(\beta_R) = \{0,n_i\} \lightning
\text{Contradiction! with \ref{three}} 
\end{equation}
For $i$ from 1 to $m$, if $r_i \in \text{span}(\beta_N)$
\begin{equation}
\text{span}(\beta_N)\cap\text{span}(\beta_R) = \{0,r_i\} \lightning
\text{Contradiction! with \ref{three}} 
\end{equation}
\begin{equation}
\therefore \beta_N\cup\beta_R \;\text{is linearly independent} \label{four}
\end{equation}
\begin{align}
\text{card}(\beta_N\cup\beta_R) & = \text{card}(\beta_N) +
\text{card}(\beta_R) - \text{card}(\beta_N\cap \beta_R)\\
&= \text{card}(\beta_N) + \text{card}(\beta_R)\\
&= k + m =n \label{five}
\end{align}
From \ref{four} and \ref{five} it follows that
\begin{equation}
\mathsf{V} = \text{span}(\beta_N\cup \beta_R)
\end{equation}
Claim: $\text{span}(\beta_N\cup\beta_R) = \text{span}(\beta_N) +
\text{span}(\beta_R) = N(\mathsf{T}) + R(\mathsf{T})$
\\$(\supseteq)$ since $\text{span}(\beta_N)$ and
$\text{span}(\beta_R)$ are both contained in $\mathsf{V}$ it follows
that
\begin{equation}
\text{span}(\beta_N) + \text{span}(\beta_R) \subseteq \mathsf{V}
\end{equation}
$(\subseteq)$ Suppose $x \in \text{span}(\beta_N\cup\beta_R)$
\begin{gather}
x = a_1v_1 + \dotsb + a_kv_k +a_{k+1}v_{k+1} \dotsb + a_{k+m}v_{k+m}\\
a_1v_1 +\dotsb + a_kv_k \in \text{span}(\beta_R)\\
a_{k+1}v_{k+1} + \dotsb +a_{k+m} \in \text{span}(\beta_N)\\
\implies x \in \text{span}(\beta_N) + \text{span}(\beta_R)
\end{gather}
\begin{equation}
\implies N(\mathsf{T}) \oplus R(\mathsf{T}) = \mathsf{V}
\end{equation}
\item Claim: $\text{rank}(\mathsf{T}^k) =
  \text{rank}(\mathsf{T}^{k+1})$ for some integer $k$
\begin{equation}
0\leq\dots \leq \text{dim}(R(\mathsf{T}^3)) \leq
\text{dim}(R(\mathsf{T}^2))\leq \text{dim}(R(\mathsf{T})) \leq n \label{1}
\end{equation}
Suppose $x \in R(\mathsf{T}^{k+1})$
\begin{gather}
\exists a \in \mathsf{V}\; \text{such that } \mathsf{T}(\mathsf{T}(a))
= x\\
\implies x \in R(\mathsf{T}^k)\\
\implies R(\mathsf{T}^k) \leq R(\mathsf{T}^{k+1}) \label{2}
\end{gather}
Since there is a lower bound 0 and an upper bound $n$ in \ref{1} it
follows that for some integer $k$
\begin{gather}
\text{dim}(R(\mathsf{T}^{k+1})) =
\text{dim}(R(\mathsf{T}^k)) \label{3}\\
\implies R(\mathsf{T}^{k+1}) = R(\mathsf{T}^k) \; (\text{by  \ref{2}
and \ref{3}}) \label{4}\\
\implies \text{rank}(\mathsf{T}^k) = \text{rank}(\mathsf{T}^{k+1})
\quad \text{for some integer } k
\end{gather}
Claim: $R\left(\mathsf{T}^{k+1}\right) = R(\mathsf{T}^m)\;\forall m \geq 1$
\\For $m=1$ by \ref{4}\\
For $m=j \rightarrow R(\mathsf{T}^{k+j}) = R(\mathsf{T}^k)$\\
For $m = j+1$
\begin{gather}
R\left(\mathsf{T}^{k+j+1}\right) =
\mathsf{T}\left(R\left(\mathsf{T}^{k+j}\right)\right) = 
\mathsf{T}\left(R\left(\mathsf{T}^k\right)\right) =
R\left(\mathsf{T}^{k+1}\right) = R\left(\mathsf{T}^k\right)\\
\implies R\left(\mathsf{T}^{k+j+1}\right) = R\left(\mathsf{T}^k\right)\\
\implies \text{rank}\left(\mathsf{T}^{k+m}\right) =\text{rank}\left(\mathsf{T}^k\right)\;
\text{for some integer } k\; \text{and for all integer } m\\
\implies \text{rank}(\mathsf{T}^{2k} = \text{rank}(\mathsf{T}^k) \;
\text{for some } k
\end{gather}
Apply the same method as in part (a) and it follows that
\begin{equation}
\mathsf{V} = R(\mathsf{T}^k)\oplus N(\mathsf{T}^k)\; \text{for some } k
\end{equation}
\end{enumerate}

