Let $\mathsf{V}$ be a vector space. Determine all linear
transformations $\mathsf{T}\colon \mathsf{V}\to\mathsf{V}$ such that
$\mathsf{T}=\mathsf{T}^2$.
\\Suppose $\mathsf{W} = \{y\colon \mathsf{T}(y) = y\}$
\\Claim: $\forall\mathsf{T}\in \mathcal{L}(\mathsf{V}), \mathsf{T}=\mathsf{T}^2 \Leftrightarrow \mathsf{T}$ is a projection of $\mathsf{W}$ along $N(\mathsf{T})$
\\Claim:$\mathsf{W}\cap N(\mathsf{T}) =\{0\}$
\\Suppose $x\in \mathsf{W}\cap N(\mathsf{T})$
\begin{gather}
\implies \mathsf{T}(x) = x \\
\implies \mathsf{T}(x) = 0\\
\implies x = 0\\
\implies \mathsf{W} \cap N(T) = \{0\}
\end{gather}
\paragraph{}$N(\mathsf{T})$ is a subspace of $\mathsf{V}$ (by theorem
2.1)
\\Claim: $\mathsf{W}$ is subspace of $\mathsf{V}$
\begin{equation}
0 \in \mathsf{W}
\end{equation}
Suppose $x,z \in \mathsf{W}$
\begin{equation}
\mathsf{T}(x+z) = \mathsf{T}(x) +\mathsf{T}(z) = x + z
\end{equation}
Suppose $x\in \mathsf{W},\; c\in F$
\begin{gather}
\mathsf{T}(cx) = c\mathsf{T}(x) = cx\\
\mathsf{W} \subseteq \mathsf{V} \;\text{by definition}
\end{gather}
Claim $\mathsf{V} = \mathsf{W} \oplus N(\mathsf{T})$
\\$(\subseteq)$ Suppose $ x \in \mathsf{V}$
\begin{gather}
\implies x = \mathsf{T}(x) + (x -\mathsf{T}(x))\\
\mathsf{T}(x) = \mathsf{T}^2(x)\\
\mathsf{T}(x) \in \mathsf{W}\\
\mathsf{T}(x-\mathsf{T}(x)) = \mathsf{T}(x) - \mathsf{T}^2(x) = 0\\
\implies x \in \mathsf{W} \oplus N(\mathsf{T})\\
\implies \mathsf{V}\subseteq\mathsf{W}
\end{gather}
$(\supseteq)$ Suppose $\mathsf{W}\subseteq\mathsf{V}$
\begin{gather}
N(\mathsf{T}) \subseteq \mathsf{V}\\
\implies \mathsf{W}\oplus N(\mathsf{T})\;\text{by closure of }
\mathsf{V}\\
\forall x \in \mathsf{V}, x = x_1 + x_2\quad\text{for some } x \in
\mathsf{W}, x_2 \in N(\mathsf{T})
\end{gather}
\begin{align}
\mathsf{T}(x) &= \mathsf{T}(x_1) + \mathsf{T}(x_2)\\
&=x_1 + 0\\
&= x_1
\end{align}
It follows that $\mathsf{T}$ is a projection of $\mathsf{W}$ along
$N(\mathsf{T})$
\\Suppose $\mathsf{T}$ is a projection of $\mathsf{W}$ along
$N(\mathsf{T})$
\\Suppose $x \in \mathsf{W}\oplus N(\mathsf{T})$
\begin{gather}
\implies x = x_1 +x_2\quad \text{for some } x_1 \in \mathsf{W}, x_2
\in N(\mathsf{T})\\
\mathsf{T}(x) = \mathsf{T}(x_1 +x_2) = \mathsf{T}(x_1)
+\mathsf{T}(x_2) = \mathsf{T}(x_1) + 0 = x_1\\
\implies \mathsf{T}(x_1) = 0\\
\mathsf{T}^2(x) = \mathsf{T}(x_1)\\
\implies \mathsf{T}^2(x) = x \\
\implies \mathsf{T}^2(x) = \mathsf{T}(x)\; \forall x \in \mathsf{V}\\
\therefore \mathsf{T}=\mathsf{T}^2
\end{gather}
