Let $\mathsf{V}$ and $\mathsf{W}$ be finite-dimensional vector spaces
and $\mathsf{T}\colon \mathsf{V} \to \mathsf{W}$ be an
isomorphism. Let $\mathsf{V}_0$ be a subspace of $\mathsf{V}$.
\begin{enumerate}[(a)]
\item Prove that $\mathsf{T}(\mathsf{V}_o)$ is a subspace of
  $\mathsf{W}$.
\item Prove that $\text{dim}(\mathsf{V}_0) = \text{dim}(\mathsf{T}(\mathsf{V}_0))$.
\end{enumerate}
Let $\mathsf{V}_0$ be a subspace of $\mathsf{V}$ 
\begin{enumerate}[(a)]
\item Claim: $0 \in \mathsf{V}_0$
\begin{gather}
0 \in \mathsf{V}_0\\
\implies \mathsf{T}(0) = 0 
\end{gather}
Claim: $\forall x , y \in \mathsf{T}(\mathsf{V}_0), x + y \in
\mathsf{T}(\mathsf{V}_0)$
\\Suppose $\beta_{\mathsf{V}_0}$ is basis for $\mathsf{V}_0$
\begin{equation}
\implies \mathsf{V}_0 = \text{span}(\beta_{\mathsf{V}_0})
\end{equation}
Suppose $x, y \in \mathsf{T}(\mathsf{V}_0)$
\begin{align}
\implies x &= \mathsf{T}(a_1u_1 + a_2u_2 + \dotsb + a_nu_n)\\
y &= \mathsf{T}(b_1u_1 + b_2u_2 + \dotsb + b_nu_n) \quad \text{for }
a_i,b_i \in F, \; u_i \in \beta_{\mathsf{V}_0}\\
\implies x &= a_1\mathsf{T}(u_1) + a_2\mathsf{T}(u_2) + \dotsb +
a_n\mathsf{T}(u_n)\\
y &= b_1\mathsf{T}(u_1) + b_2\mathsf{T}(u_2) +\dotsb +
b_n\mathsf{T}(u_n)\\
\implies x +y &= (a_1+b_1)\mathsf{T}(u_1) + (a_2 +b_2)\mathsf{T}(u_2) +
\dotsb + (a_n+b_n)\mathsf{T}(u_n)\\
&= \mathsf{T}((a_1 +b_2)u_1 + (a_2+b_2)u_2 + \dotsb + (a_n + b_n)u_n)
\end{align}
\begin{equation}
\implies x + y \in \mathsf{T}(\text{span}(\beta_{\mathsf{V}_0}))
\end{equation}
Claim: $\forall x \in \mathsf{T}(\mathsf{V}_0)$ and $\forall c \in F,
cx \in \mathsf{T}(\mathsf{V}_0)$
\\Suppose $x \in \mathsf{T}(\mathsf{V}_0)$ such that
\begin{equation}
x = \mathsf{T}(a_1u_1 + a_2u_2 + \dotsb + a_nu_n)\quad \text{for }
u_i\in \beta_{\mathsf{V}_0}, a_i \in F
\end{equation}
\begin{equation}
\implies x = a_1\mathsf{T}(u_1) + a_2\mathsf{T}(u_2) + \dotsb + a_n\mathsf{T}(u_n)
\end{equation}
\begin{align}
cx &= c\left(a_1\mathsf{T}(u_1) + a_2\mathsf{T}(u_2) + \dotsb +
  a_n\mathsf{T}(u_n) \right)\\
&= ca_1\mathsf{T}(u_1) + ca_2\mathsf{T}(u_2) +\dotsb +
ca_n\mathsf{T}(u_n)\\
&= \mathsf{T}(ca_1u_1 + ca_2u_2 + \dotsb + ca_nu_n)
\end{align}
\begin{equation}
\implies cx \in \mathsf{T}(\text{span}(\beta_{\mathsf{V}_0}))
\end{equation}
$\mathsf{T}(\mathsf{V}_0) \subseteq \mathsf{W}$ by the definition of
$\mathsf{T}$. It follows that $\mathsf{T}(\mathsf{V}_0)$ is a subspace
of $\mathsf{W}$.
\item Claim: $\text{dim}(\mathsf{V}_0) = \text{dim}(\mathsf{T}(\mathsf{V}_0$))
\\Suppose $\beta_{\mathsf{V}_0}$ is a basis of $\mathsf{V}_0$
\paragraph{Lemma:} $\mathsf{T}(\beta_{\mathsf{V}_0}) \; \text{is a
  basis of } \mathsf{T}(\mathsf{V}_0)$

% \\Claim: $\text{card}(\beta_{\mathsf{V}_0}) =
% \text{card}(\mathsf{T}(\beta_{\mathsf{V}_0}))$
% \paragraph{} $\mathsf{T}$ is an isomorphism. Equivalently it also
% invertible and 1-1. Therefore it follows that for every $x\in
% \mathsf{T}(\beta_{\mathsf{V}_0})$ there exists a unique vector $y \in
% \beta_{\mathsf{V}_0}$ such that $\mathsf{T}(y) =x$
%\\Claim: $\mathsf{T}(\beta_{\mathsf{V}_0})$ is a basis of
%$\mathsf{T}(\mathsf{V}_0)$
%\begin{equation}
%\mathsf{T}(\beta_{\mathsf{V}_0})\;\text{is a basis of }
%\mathsf{T}(\mathsf{V}_0) \Leftrightarrow
Claim: $\text{span}(\mathsf{T}(\beta_{\mathsf{V}_0})) = \mathsf{T}(\text{span}(\beta_{\mathsf{V}_0}))$
%\end{equation}
\\$(\subseteq)$ Suppose $x \in
\text{span}(\mathsf{T}(\beta_{\mathsf{V}_0}))$
\begin{align}
x &= a_1\mathsf{T}(u_1) + a_2\mathsf{T}(u_2) + \dotsb +
a_n\mathsf{T}(u_n)\\
&= \mathsf{T}(a_1u_1 +a_2u_2 + \dotsb + a_nu_n)\quad \text{for } u_i
\in \beta_{\mathsf{V}_0}, a_i \in F
\end{align}
\begin{gather}
a_1u_1 +a_2u_2 +\dotsb + a_nu_n \in
\text{span}(\beta_{\mathsf{V}_0})\\
\implies x \in \mathsf{T}(\text{span}(\beta_{\mathsf{V}_0}))
\end{gather}
$(\supseteq)$ Suppose $x\in
\mathsf{T}(\text{span}(\beta_{\mathsf{V}_0}))$ such that 
\begin{align}
x &= \mathsf{T}(a_1u_1 + a_1u_2 +\dotsb +
a_nu_n)\quad\text{for }a_i \in F, u_i \in
\beta_{\mathsf{V}_0}\\
&= a_1\mathsf{T}(u_1) + a_2\mathsf{T}(u_2) + \dotsb + a_n\mathsf{T}(u_n)
\end{align}
\begin{equation}
\implies x \in \text{span}(\mathsf{T}(\beta_{\mathsf{V}_0}))
\end{equation}
Claim: $\mathsf{T}(\beta_{\mathsf{V}_0})$ is linearly independent
\begin{gather}
\beta_{\mathsf{V}_0}\; \text{is linearly independent and } \mathsf{T}
\; \text{is 1-1}\\
\implies \mathsf{T}(\beta_{\mathsf{V}_0})\; \text{is linearly
  independent by HW.2.1.14.a} 
\end{gather}
\newpage{}
Claim: $\text{card}(\beta_{\mathsf{V}_0}) =
\text{card}(\mathsf{T}(\beta_{\mathsf{V}_0}))$
\paragraph{} $\mathsf{T}$ is an isomorphism. Equivalently it also
invertible and 1-1. Therefore it follows that for every $x\in
\mathsf{T}(\beta_{\mathsf{V}_0})$ there exists a unique vector $y \in
\beta_{\mathsf{V}_0}$ such that $\mathsf{T}(y) =x$
\begin{equation}
\therefore \text{dim}(\beta_{\mathsf{V}_0}) = \text{dim}(\mathsf{T}(\beta_{\mathsf{V}_0}))
\end{equation}
\end{enumerate}
