For each of the following linear transformations $\mathsf{T}$,
determine whether $\mathsf{T}$ is invertible and justify your answer.
\begin{enumerate}[(a)]
\setcounter{enumii}{1}
\item $\mathsf{T}\colon \mathsf{T}^2 \to \mathsf{R}^3$ defined by
  $\mathsf{T}(a_1,a_2) = (3a_1-2a_2,a_2,4a_1)$
\\Claim: $\mathsf{T}$ is 1-1
\\Suppose $x,y\in \mathbb{R}^2$ such that $x=(a_1,a_2), y= (a_3,a_4)$
and $\mathsf{T}(x)=\mathsf{T}(y)$ for $a_i \in \mathbb{R}$
\begin{equation}
(3a_1-a_2,a_2,4a_1) = (3a_3-a_4,a_4,4a_3)
\end{equation}
\begin{align}
\implies 3a_1-a_2 &= 3a_3-a_4\\
a_2&= a_4\\
4a_1&= 4a_3
\end{align}
\begin{align}
\implies a_1&=a_3\\
a_2&=a_4
\end{align}
\begin{equation}
\implies x=y
\end{equation}
Claim: $\mathsf{T}$ is onto
\\Suppose $x\in\mathbb{R}^3$ such that $x=(b_1,b_2,b_3)$ for $b_i\in
\mathbb{R}$
\\Let $b_2=a_2,b_3=4a_1,b_1=(\frac{3}{4}b_3-b_2)$
\begin{gather}
\implies (b_1,b_2,b_3) = (2a_1-a_2,a_2,4a_1)\\
\implies x\in R(\mathsf{T})\\
R(\mathsf{T}) \subseteq \mathsf{M}_{n\times n}(\mathbb{R})\;\text{by
  def of}\; \mathsf{T}\\
\notag \therefore \mathsf{T}\;\text{is invertible}
\end{gather}
\setcounter{enumii}{4}
\item $\mathsf{T}\colon \mathsf{M}_{2\times 2}(\mathbb{R}) \to \mathsf{P}_2(\mathbb{R})$ defined by $\mathsf{T}\begin{pmatrix}a&b\\c&d
  \end{pmatrix} = a + 2bx + (c+d)x^2$
\\Claim: $\mathsf{T}$ is not 1-1
\\Suppose $x,y \in \mathsf{M}_{2\times 2}(\mathbb{R})$ such that
\begin{align}
x = \begin{pmatrix}0 & 0\\ 1 & 4\end{pmatrix}& & y = \begin{pmatrix} 0
  & 0\\ 2 & 3\end{pmatrix}
\end{align}
\begin{equation}
\implies x \neq y
\end{equation}
\begin{align}
\mathsf{T}(x) &= (0\cdot 1) + (2\cdot 0) x + (1+4)x^2 = 5x^2\\
\mathsf{T}(y) &= (0\cdot 1) + (2\cdot 0) x + (3+2)x^2 = 5x^2
\end{align}
\begin{equation*}
\therefore \mathsf{T}\;\text{is not invertible}
\end{equation*}
\item $\mathsf{T}\colon \mathsf{M}_{2\times 2}(\mathbb{R}) \to
  \mathsf{M}_{2\times 2}(\mathbb{R})$ defined by $\mathsf{T}\begin{pmatrix}a&b\\c&d
  \end{pmatrix} = \begin{pmatrix} a+b& a\\ c & c+d
  \end{pmatrix}$.
\\Claim: $\mathsf{T}$ is 1-1
\\Suppose $x,y \in \mathsf{M}_{2\times 2}(\mathbb{R})$ such that
\begin{align}
x = \begin{pmatrix}a & b\\ c & d\end{pmatrix} & & y = \begin{pmatrix}e &
  f\\ g & h\end{pmatrix}
\end{align}
Suppose $\mathsf{T}(x) = \mathsf{T}(y)$ for $a,b,c,\dotsc,h \in
\mathbb{R}$
\begin{equation}
\implies 
\begin{pmatrix}
a+b & a \\
c & c +d 
\end{pmatrix}
=
\begin{pmatrix}
e +f & e \\
g & g + h
\end{pmatrix}
\end{equation}
\begin{align}
\implies a + b &= e + f \\
a &= e\\
c &= g\\
c + d &= g + h
\end{align}
\begin{align}
\implies a &= e\\
b &= f\\
c &= g\\
d &= h
\end{align}
\begin{equation}
\implies x=y
\end{equation}
Claim: $\mathsf{T}$ is onto
\\Suppose $x\in\mathsf{M}_{2\times 2}(\mathbb{R})$ such that
\begin{equation}
x = 
\begin{pmatrix} 
a & b\\
c & d
\end{pmatrix}
\quad \text{for}\; a,b,c,d \in \mathbb{R}
\end{equation}
Let $e,f,g,h \in \mathbb{R}$ such that 
\begin{align}
e = b & & f &= e +a \\
g = c & & h &= -g +d
\end{align}
\begin{gather}
x =
\begin{pmatrix}
e +f & e\\
g & g + h
\end{pmatrix}\\
\implies x \in R(\mathsf{T})\\
R(T) \subseteq \mathsf{M}_{2\times 2}(\mathbb{R})\; \text{by definition
  of}\; \mathsf{T}\\
\notag \therefore \mathsf{T}\; \text{is invertible}
\end{gather}
\end{enumerate}
