Let $\mathsf{T}\colon\mathsf{V}\to\mathsf{W}$ be a linear
transformation from an $n$-dimensional vector space $\mathsf{V}$ to an
m-dimensional vector space $\mathsf{W}$  Let $\beta$ and $\gamma$ be
ordered bases for $\mathsf{V}$ and $\mathsf{W}$ respectively. Prove
that $\text{rank}(\mathsf{T}) = \text{rank}(\mathsf{L}_A)$ and that
$\text{nullity}(\mathsf{T}) = \text{nullity}(\mathsf{L}_A)$, where $A = [\mathsf{T}]^\gamma_\beta$.
\\Claim: $\text{nullity}(\mathsf{T}) = \text{nullity}(\mathsf{L}_A)$
\paragraph{}$N(\mathsf{T})$ is a subspace of $\mathsf{V}$. This implies
that $\phi_\beta(N(\mathsf{T}))$ is a subspace of $\mathsf{F}^n$ and
$\text{dim}(N(\mathsf{T})) = \text{dim}(\phi_\beta(N(\mathsf{T})))$ by HW.2.4.17
\\Claim: $\phi_\beta(N(\mathsf{T})) = N(\mathsf{L}_A)$
\\$(\subseteq)$ Suppose $y \in \phi_\beta(N(\mathsf{T}))$
\begin{gather}
\implies y = \phi_\beta(x)\\
\implies \mathsf{L}_A = \mathsf{L}_A\phi_\beta(x) =
\phi_\gamma\mathsf{T}(x) = \phi_\gamma(0) =0 \\
y \in N(\mathsf{L}_A)
\end{gather}
\\$(\supseteq)$ Suppose $y \in N(\mathsf{L}_A)$
\begin{gather}
N(\mathsf{L}_A) \subseteq \mathsf{F}^n\;\text{by definition of }
N(\mathsf{L}_A)\\
\implies \forall y \in N(\mathsf{L}_A), \exists ! x\in \mathsf{V}
\;\text{such that } \phi_\beta(x) = y\\
\notag \because \phi_\beta\; \text{is an isomorphism}\\
%\end{gather}
%\begin{gather}
\mathsf{L}_A(y) = \mathsf{L}_A(\phi_\beta(x)) =0 \\
\mathsf{L}_A\phi_\beta = \phi_\gamma\mathsf{T}\\
\implies \phi_\gamma(\mathsf{T}(x)) = 0
\implies \mathsf{T}(x) =0 \\
\notag \because \phi_\gamma\; \text{is an isomorphism}\\
\therefore y \in \phi_\beta(N(\mathsf{T}))\\
% N(\phi_\gamma) = \{0\}\\
\phi_\beta(N(\mathsf{T})) = N(\mathsf{L}_A) \implies \text{dim}(\phi_\beta(N(\mathsf{T}))) = \text{dim}(N(\mathsf{L}_A))=\text{dim}(N(\mathsf{T}))\\
\therefore \text{nullity}(\mathsf{T}) = \text{nullity}(\mathsf{L}_A)
\end{gather}
\newpage{}
Claim: $\text{rank}(\mathsf{T}) = \text{rank}(\mathsf{L}_A)$
\paragraph{} $R(\mathsf{T})$ is a subspace of $\mathsf{W}$. This
implies that $\phi_\gamma(R(\mathsf{T}))$ is subspace of $\mathsf{W}$
and $\text{dim}(R(\mathsf{T})) =
\text{dim}(\phi_\gamma(R(\mathsf{T}))$ by HW.2.4.17
\\Claim: $\phi_\gamma(R(\mathsf{T})) = R(\mathsf{L}_A)$
\\$(\subseteq)$ Suppose $x \in\phi_\gamma(R(\mathsf{T}))$
\begin{gather}
\implies x \in \phi_\gamma(y)\quad \text{for some } y \in
R(\mathsf{T})\\
\implies y \in \mathsf{T}(z)\quad \text{for some } z \in \mathsf{V}
\end{gather}
\begin{gather}
\phi_\gamma(\mathsf{T}(z)) = (\phi_\gamma\mathsf{T})(x)\\
\phi_\gamma\mathsf{T} = \mathsf{L}_A\phi_\beta
\end{gather}
\begin{align}
\implies x &= (\mathsf{L}_A\phi_\beta)(z)\\
&= \mathsf{L}_A(w)\quad \text{for some } w \in \mathsf{F}^n
\end{align}
\begin{equation}
\implies x \in R(\mathsf{L}_A)
\end{equation}
$(\supseteq)$ Suppose $x \in R(\mathsf{L}_A)$ 
\begin{gather}
\implies x = [\mathsf{T}]_\beta^\gamma\phi_\beta(z)\quad \text{for
  some } z \in \mathsf{V}\\
\implies x = \mathsf{L}_A(\phi_\beta(z)) = (\mathsf{L}_A\phi_\beta)(z)
= \phi_\gamma\mathsf{T}(z)
\end{gather}
\begin{gather}
\mathsf{T}(z) \in R(\mathsf{T})\\
\implies x \in \phi_\gamma(R(\mathsf{T}))\\
\phi_\gamma(R(\mathsf{T})) = R(\mathsf{L}_A) \implies
\text{dim}(\phi_\gamma(R(\mathsf{T}))) = \text{dim}(R(\mathsf{L}_A)) =
\text{dim}(R(\mathsf{T}))\\
\therefore \text{rank}(\mathsf{T}) = \text{rank}(\mathsf{L}_A)
\end{gather}
