Let $A$ be invertible. Prove that $A^t$ is invertible and $(A^t)^{-1}
= (A^{-1})^t$.
\\Claim: $A^t$ is invertible
\begin{equation}
\implies (AB)^t =(BA)^t = I^t = I
\end{equation}
\paragraph{Lemma:} $(AB)^t = B^tA^t$
\begin{align}
(AB)^t_{ij} &= (AB)^{}_{ji} \\
&= \sum\limits_{k=1}^nA_{jk}B_{kj}\\
(B^tA^t)_{ij} &= \sum\limits_{k=1}^nB^t_{ik}A^t_{kj}\\
&=\sum\limits_{k=1}B_{kj}A_{jk}\\
&=\sum\limits_{k=1}^nA_{jk}B_{kj}
\end{align}
\begin{equation}
\implies B^tA^t = A^tB^t = I
\end{equation}
Claim: $(A^{-1})^t = (A^t)^{-1}$
\begin{equation}
B=A^{-1}
\end{equation}
\begin{equation}
(A^t)^{-1} = B^t = (A^{-1})^t
\end{equation}
