For each matrix $A$ and ordered basis $\beta$, find
$[\mathsf{L}_A]_\beta$. Also find an invertible matrix $Q$ such that
$[\mathsf{L}_A]_\beta = Q^{-1}AQ$.
\begin{enumerate}[(a)]
\item[(b)] $A = \begin{pmatrix}1&2\\2&1
  \end{pmatrix}$ and $\beta =\left\{\begin{pmatrix}1\\1\
    \end{pmatrix},\begin{pmatrix}1\\-1
    \end{pmatrix}
  \right\}$
\begin{align}
v_1 =\begin{pmatrix} 1\\ 1 \end{pmatrix} & & v_2 =\begin{pmatrix} 1 \\
  -1 \end{pmatrix}
\end{align}
\begin{gather}
\mathsf{L}_{A}(v_1) = \begin{pmatrix} 1 & 2\\ 2 &
  1\end{pmatrix}\begin{pmatrix}1\\1\end{pmatrix}
= \begin{pmatrix}3\\3\end{pmatrix} = 3\begin{pmatrix}1\\1\end{pmatrix}
+ 0\begin{pmatrix}1\\-1\end{pmatrix}\\
\implies \left[\mathsf{L}_A(v_1)\right]_\beta = \begin{pmatrix}0\\3\end{pmatrix}
\end{gather}
\begin{gather}
\mathsf{L}_A(v_2) =\begin{pmatrix}1 & 2\\2
  &1\end{pmatrix}\begin{pmatrix}1\\-1\end{pmatrix}
= \begin{pmatrix}-1\\1\end{pmatrix} =
0\begin{pmatrix}1\\1\end{pmatrix} +
-1\begin{pmatrix}1\\-1\end{pmatrix}\\
\implies \left[\mathsf{L}_A(v_1)\right]_\beta = \begin{pmatrix}0\\-1\end{pmatrix}
\end{gather}
\begin{equation}
\implies [\mathsf{L}_A] = \begin{pmatrix}3&0\\0 & -1\end{pmatrix}
\end{equation}
\begin{equation}
Q = \begin{pmatrix}1 & 1 \\ 1 & -1\end{pmatrix}
\end{equation}
\begin{equation}
\begin{gmatrix}[left]
1 & 1&\\
1 & -1 &
\end{gmatrix}
\begin{gmatrix}[right]
1 & 0\\
0 & 1
\rowops
\add[-1]{0}{1}
\mult{1}{\cdot -\frac{1}{2}}
\add[-1]{1}{0}
\end{gmatrix}
\rightarrow
\begin{gmatrix}[left]
1 & 0&\\
0 & 1&
\end{gmatrix}
\begin{gmatrix}[right]
^1/_2 & ^1/_2\\
^1/_2  & ^{-1}/_2
\end{gmatrix}
\end{equation}
\begin{equation}
\implies Q^{-1} = \begin{pmatrix}
^1/_2 & ^1/_2\\
^1/_2  & ^{-1}/_2
\end{pmatrix}
\end{equation}
\item[(c)] $A = \begin{pmatrix}1&1&-1\\2&0&1\\1&1&0
    \end{pmatrix}$
    and 
$\beta = \left\{\begin{pmatrix}1\\1\\1
    \end{pmatrix}, \begin{pmatrix}1\\0\\1
    \end{pmatrix},\begin{pmatrix}1\\1\\2
    \end{pmatrix}\right\}$
\begin{align}
v_1 = \begin{pmatrix}1\\1\\1\end{pmatrix} & & v_2 = \begin{pmatrix}1
  \\ 0 \\1\end{pmatrix} & & v_3 = \begin{pmatrix}1\\1\\2\end{pmatrix}
\end{align}
\begin{align}
\mathsf{L}_A(v_1)
&= \begin{pmatrix}1&1&-1\\2&0&1\\1&1&0\end{pmatrix}\begin{pmatrix}1\\0\\1\end{pmatrix}
= \begin{pmatrix}1\\3\\2\end{pmatrix}\\
\mathsf{L}_A(v_2) &= \begin{pmatrix}1 & 1 & -1\\2&0&-1\\1& 1
  &0\end{pmatrix} \begin{pmatrix}1\\0\\1\end{pmatrix}
= \begin{pmatrix}0\\3\\1\end{pmatrix}\\
\mathsf{L}_A(v_3)
&= \begin{pmatrix}1&1&-1\\2&0&1\\1&1&0\end{pmatrix}\begin{pmatrix}1\\1\\2\end{pmatrix}
= \begin{pmatrix}0\\4\\2\end{pmatrix}
\end{align}
\begin{equation}
\begin{pmatrix}1\\3\\2\end{pmatrix}=
a\begin{pmatrix}1\\1\\1\end{pmatrix} +
b\begin{pmatrix}1\\0\\1\end{pmatrix} +
c\begin{pmatrix}1\\1\\2\end{pmatrix}
\end{equation}
\begin{align*}
& a+b+c &=1 & & a+b +c &=1 & & b &= -2\\
\implies& a +c &=3 &\implies& a+c &= 3 &\implies& a &=2\\
& a+b + 2c &= 2 & & c &=1 & &c &=1
\end{align*}
\begin{equation}
\implies \left[\mathsf{L}_A(v_1)\right]_\beta = \begin{pmatrix}2\\-2\\1\end{pmatrix}
\end{equation}

\begin{equation}
\begin{pmatrix}0\\3\\1\end{pmatrix}=
a\begin{pmatrix}1\\1\\1\end{pmatrix} +
b\begin{pmatrix}1\\0\\1\end{pmatrix} +
c\begin{pmatrix}1\\1\\2\end{pmatrix}
\end{equation}
\begin{align*}
& a+b+c &=0 & & a+b +c &=0 & & b &= -3\\
\implies& a +c &=3 &\implies& a &= 2 &\implies& a &=2\\
& a+b + 2c &= 1 & & c &=1 & &c &=1
\end{align*}
\begin{equation}
\implies \left[\mathsf{L}_A(v_2)\right]_\beta = \begin{pmatrix}2\\-3\\1\end{pmatrix}
\end{equation}

\begin{equation}
\begin{pmatrix}0\\4\\2\end{pmatrix}=
a\begin{pmatrix}1\\1\\1\end{pmatrix} +
b\begin{pmatrix}1\\0\\1\end{pmatrix} +
c\begin{pmatrix}1\\1\\2\end{pmatrix}
\end{equation}
\begin{align*}
& a+b+c &=0 & & a+b +c &=0 & & b &= -4\\
\implies& a +c &=4 &\implies& a &= 2 &\implies& a &=2\\
& a+b + 2c &= 2 & & c &=2 & &c &=2
\end{align*}
\begin{equation}
\implies \left[\mathsf{L}_A(v_3)\right]_\beta = \begin{pmatrix}2\\-4\\2\end{pmatrix}
\end{equation}
\begin{equation}
\implies [\mathsf{L}_A]_\beta = \begin{pmatrix}2&2&2\\-2&-3&-4\\1&1&2\end{pmatrix}
\end{equation}
\begin{equation}
Q = \begin{pmatrix}
1 & 1 & 1\\
1 & 0 & 1\\
1 & 1 & 2
\end{pmatrix}
\end{equation}
\begin{equation*}
\begin{gmatrix}[left]
1 & 1 & 1&\\
1 & 0 & 1&\\
1 & 1 & 2&
\end{gmatrix}
\begin{gmatrix}[right]
1 & 0 & 0\\
0 & 1 & 0\\
0 & 0 & 1
\rowops
\add[-1]{0}{1}
\add[-1]{0}{2}
\add[1]{1}{0}
\add[1]{2}{0}
\mult{1}{\cdot -1}
\end{gmatrix}
\end{equation*}
\begin{equation}
\rightarrow
\begin{gmatrix}[left]
1 & 0 & 0& \\
0 & 1 & 0&\\
0 & 0 & 1&
\end{gmatrix}
\begin{gmatrix}[right]
1 & 1 & -1\\
1 & -1 & 0\\
-1 & 0 & 1
\end{gmatrix}
\end{equation}
\begin{equation}
\implies Q^{-1} = \begin{pmatrix}
1 & 1 & -1\\
1 & -1 & 0\\
-1 & 0 & 1
\end{pmatrix}
\end{equation}
\end{enumerate}
