For 
\[
A = \begin{pmatrix}
1 & 4 \\
2 & 3
\end{pmatrix} \in \mathsf{M}_{n\times n}(\mathbb{R}),
\]
find an expression for $A^n,$ where $n$ is an arbitrary positive
integer.
\begin{align}
\det{\begin{pmatrix}
1 - \lambda & 4\\
2 & 3-\lambda 
\end{pmatrix}
} &= (1-\lambda)(3-\lambda)-8 = 0\\
&= (\lambda-5)(\lambda+1) = 0 
\end{align}
\begin{align}
\implies \lambda_1 &= 5\\
\lambda_2 &= -1
\end{align}
\begin{itemize}
\item For $\lambda_1 = 5$
\begin{equation}
\begin{pmatrix}
-4 & 4\\
2 & -2
\end{pmatrix}
\begin{pmatrix}
x_1 \\ x_2
\end{pmatrix}=
\begin{pmatrix}
0\\0
\end{pmatrix}
\leadsto 
\begin{pmatrix}
0 & 0\\
1 & -1
\end{pmatrix}
\begin{pmatrix}
x_1 \\ x_2
\end{pmatrix}=
\begin{pmatrix}
0\\0
\end{pmatrix}
\end{equation}
\begin{gather}
\implies x_1 = x_2\\
\implies S_1 = \left\{z\begin{pmatrix}1\\1\end{pmatrix}\colon z \in
  \mathbb{R}\right\}\\
\implies \text{ eigenvector corresponding to } \lambda_1 =5 \text{ is
} \begin{pmatrix}1\\1\end{pmatrix}
\end{gather}
\item For $\lambda_2 = -1$
\begin{equation}
\begin{pmatrix}
2 & 4\\
2 & 4
\end{pmatrix}
\begin{pmatrix}
x_1 \\ x_2
\end{pmatrix}
=
\begin{pmatrix}
0 \\ 0
\end{pmatrix}
\leadsto
\begin{pmatrix}
1 & 2\\
0 & 0
\end{pmatrix}
\begin{pmatrix}
2 & 4\\
2 & 4
\end{pmatrix}
\begin{pmatrix}
x_1 \\ x_2
\end{pmatrix}
=
\begin{pmatrix}
0 \\ 0
\end{pmatrix}
\end{equation}
\begin{gather}
\implies x_1 = -2x_2\\
\implies S_2 = \left\{z\begin{pmatrix}-2\\1\end{pmatrix}\colon z \in
  \mathbb{R}\right\}\\
\implies \text{ eigenvector corresponding to } \lambda_2 =-1 \text{ is
} \begin{pmatrix}-2\\1\end{pmatrix}
\end{gather}
\end{itemize}
 Let $Q = \begin{pmatrix}
1 & -2 \\
1 & 1
\end{pmatrix}$
\begin{equation}
\begin{gmatrix}[left]
1 & -2 & \\
1 & 1 & 
\end{gmatrix}
\begin{gmatrix}[right]
1 & 0 \\
0 & 1
\end{gmatrix}\leadsto
\begin{gmatrix}[left]
1 & 0 &\\
0 & 1 &
\end{gmatrix}
\begin{gmatrix}[right]
\mfrac{1}{3} & \mfrac{2}{3}\\
\mfrac{-1}{3} & \mfrac{1}{3}
\end{gmatrix}
\end{equation}
\begin{gather}
\implies Q^{-1} = 
\begin{pmatrix}
\mfrac{1}{3} & \mfrac{2}{3}\\
\mfrac{-1}{3} & \mfrac{1}{3}
\end{pmatrix}\\
D = Q^{-1}AQ = \begin{pmatrix}
5 & 0\\
0 & -1
\end{pmatrix}\\
\implies A = QDQ^{-1}
\end{gather}
\begin{align}
\implies A^n &= (QDQ^{-1})^n\\
&= QD^nQ^{-1}\\
&= \begin{pmatrix}
1 & -2\\
1 & 1
\end{pmatrix}
\begin{pmatrix}
5^n & 0\\
0 & (-1)^n
\end{pmatrix}
\begin{pmatrix}
\mfrac{1}{3} & \mfrac{2}{3}\\
\mfrac{-1}{3} & \mfrac{1}{3}
\end{pmatrix}
\end{align}
