Let $f(x)$ be a polynomial with coefficients from a field $F,$ and let
$\mathsf{T}$ be a linear operator on a vector space $\mathsf{V}$ over
$F$. Then the following statements are true
\begin{enumerate}
\item $f(\mathsf{T})$ is a linear operator on $\mathsf{V}.$
\item If $\beta$ is a finite ordered basis for $\mathsf{V}$ and $A =
  [\mathsf{T}]_\beta,$ then $[f(\mathsf{T})]_\beta = f(A).$
\end{enumerate}

Suppose $f(x)$ is a polynomial with coefficients in $F$

Suppose $\mathsf{T} \in \mathcal{V}$ and $\mathsf{V}$ is a vector
space over $F.$
\begin{enumerate}
\item Claim: $f(\mathsf{T})$ is a linear operator on $\mathsf{V}.$
\begin{align}
f(x) &= a_nx^n + a_{n-1}x^{n-1} + \dotsb + a_1x + a_0 \\
f(\mathsf{T}) &= a_n\mathsf{T}^n + a_{n-1}\mathsf{T}^{n-1} + \dotsb +
a_1\mathsf{T} + a_0\mathsf{I}_\mathsf{V}
\end{align}
\paragraph{Lemma: } $\mathsf{T}^n \in \mathcal{L}(\mathsf{V})\; \forall
n \in \mathbb{Z}^+.$

Suppose $y,z \in \mathsf{V}.$

Suppose $n=1$
\begin{equation}
\mathsf{T}(az+y) = a\mathsf{T}(z) +\mathsf{T}(y)
\end{equation}
Suppose true for $1\leq n\leq k.$

Suppose $n=k+1$
\begin{align}
\mathsf{T}^{k+1}(az+y) &= \mathsf{T}(\mathsf{T}^k(az+y))\\
&= \mathsf{T}(a\mathsf{T}^k(z) + \mathsf{T}(y))\\
&= a\mathsf{T}^{k+1}(z) + \mathsf{T}^{k+1}(y) \\ & & \qedsymbol\notag
\end{align}
\begin{multline}
\therefore f(\mathsf{T}(az+y)) = a_n\mathsf{T}^n(az+y)
+a_{n-1}\mathsf{T}^{n-1}(az+y) +\dotsb + \\  {}+a_1\mathsf{T}(az +y) +
a_0(az+y)
\end{multline}
\begin{multline}
f(\mathsf{T}(az+y)) = a_n(a\mathsf{T}^n(z) + \mathsf{T}^n(y)) +
a_{n-1}(a\mathsf{T}^{n-1}(z) +\mathsf{T}^{n-1}(y)) + \dotsb + \\ {} +
a_1(a\mathsf{T}(z) +\mathsf{T}(y)) +a_0(az +y)
\end{multline}
\begin{multline}
f(\mathsf{T}(az+y)) = a(a_n\mathsf{T}^n(z)+a_{n-1}\mathsf{T}^{n-1}(z)
+ \dotsb + a_1\mathsf{T}(z) +a_oz) + \\
+ (a_n\mathsf{T}^n(y)+a_{n-1}\mathsf{T}^{n-1}(y)
+ \dotsb + a_1\mathsf{T}(y) +a_oy)
\end{multline}
\begin{equation}
f(\mathsf{T}(az+y)) = af(\mathsf{T})(z) + f(\mathsf{T})(y) \in \mathsf{V}
\end{equation}
\begin{equation}
\implies f(\mathsf{T}) \in \mathcal{L}(\mathsf{V})
\end{equation}
\item Claim: If $\beta$ is a finite ordered basis for $\mathsf{V}$ and
  $A=[\mathsf{T}]_\beta,$ then $\left[f(\mathsf{T})\right]_\beta = f(A).$
\begin{equation}
f(\mathsf{T}) = a_n\mathsf{T}^n +a_{n-1}\mathsf{T}^{n-1}+\dotsb
+a_1\mathsf{T} +a_0\mathsf{I}_\mathsf{V}
\end{equation}
\begin{align}
\implies\left[f(\mathsf{T})\right]_\beta &= \left[a_n\mathsf{T}^n +a_{n-1}\mathsf{T}^{n-1}+\dotsb
+a_1\mathsf{T} +a_0\mathsf{I}_\mathsf{V}\right]_\beta\\
&= a_n\left[\mathsf{T}^n\right]_\beta
a_{n-1}\left[\mathsf{T}^{n-1}\right]_\beta + \dotsb +
a_1\left[\mathsf{T}\right]_\beta
  +a_0\left[\mathsf{I}_\mathsf{V}\right]_\beta\\
&= a_n\left(\left[\mathsf{T}\right]_\beta\right)^n
+a_{n-1}\left(\left[\mathsf{T}\right]_\beta\right)^{n-1} + \dotsb +
a_1\left[\mathsf{T}\right]_\beta + a_0\mathsf{I}_\mathsf{V}\\
&= a_nA^n +a_{n-1}A^{n-1} +\dotsb + a_1A +a_0\\
&= f(A)
\end{align}
\end{enumerate}
