Prove that if $\mathsf{V}=\mathsf{W}\oplus \mathsf{W}^\perp$ and
$\mathsf{T}$ is the projection on $\mathsf{W}$ along
$\mathsf{W}^\perp,$ then $\mathsf{T}=\mathsf{T}^*.$

Suppose $\mathsf{V} = \mathsf{W}\oplus \mathsf{W}^\perp$ and
$\mathsf{T}$ is a projection on $\mathsf{W}$ along $\mathsf{W}^\perp$

Suppose $x,y \in \mathsf{V}$ such that $x=x_1+x_2$ and $y=y_1+y_2$
where $x_1,y_1 \in \mathsf{W}$ and $x_2,y_2 \in \mathsf{W}^\perp$

\begin{align}
\langle \mathsf{T}(x), y \rangle &= \langle x,\mathsf{T}^*(y)\\
&=\langle x,y_1+y_2\rangle\\
&=\langle x_1,y_2 \rangle + \langle x_1,y_2\rangle\\
&= \langle x_1,y_1 \rangle
\end{align}
\begin{align}
\langle x, \mathsf{T}(y) \rangle &= \langle \mathsf{T}^*(x), y
\rangle\\
&= \langle x_1+x_2,y_1 \rangle\\
&= \langle x_1,y_1 \rangle + \langle x_2,y_2 \rangle \\
&=\langle x_1,y_1 \rangle
\end{align}
\begin{gather}
\implies \langle x, \mathsf{T}(y) \rangle = \langle x, \mathsf{T}^*(y)
\rangle \quad \forall x \in \mathsf{V}\\
\implies \mathsf{T}(y) = \mathsf{T}^*(y) \quad \forall y \in \mathsf{V}
\end{gather}
