Assume that $\mathsf{T}$ is a linear operator on a complex (not
necessarily finite-dimensional) inner product space $\mathsf{V}$ with
an adjoint $\mathsf{T}^*.$ Prove the following results.
\begin{enumerate}
\item If $\mathsf{T}$ is self-adjoint, then $\langle
  \mathsf{T}(x),x\rangle$ is real for all $x \in \mathsf{V}.$
\item If $\mathsf{T}$ satisfies $\langle \mathsf{T}(x),x \rangle = 0$
  for all $x \in \mathsf{V},$ then $\mathsf{T} = \mathsf{T}_0.$\\
\item If $\langle \mathsf{T}(x),x \rangle$ is real for all $x \in
  \mathsf{V},$ then $\mathsf{T} = \mathsf{T}^*.$
\end{enumerate}
\begin{enumerate}
\item Claim: If $\mathsf{T}$ is self-adjoint then $\langle
  \mathsf{T}(x),x \rangle$ is real $\forall x \in \mathsf{V}$
\begin{gather}
\langle \mathsf{T}(x),x \rangle = \langle x, \mathsf{T}^*(x) \rangle =
\langle x, \mathsf{T}(x) \rangle\\
\overline{\langle \mathsf{T}(x),x \rangle} = \langle x, \mathsf{T}(x)
\rangle\\
\implies \langle \mathsf{T}(x),x \rangle = \overline{\langle
  \mathsf{T}(x),x \rangle}\\
\notag \implies \langle\mathsf{T}(x), x \rangle \text{ is real}
\end{gather}
\item Suppose $\mathsf{T}$ satisfies $\langle \mathsf{T}(x),x \rangle =0 \;
\forall x \in \mathsf{V}$ 

Claim: $\mathsf{T} = \mathsf{T}_0$

Let $z = x + y$
\begin{align}
\langle \mathsf{T}(z),z\rangle &= \langle \mathsf{T}(x+y),x+y\rangle
\\
&= \langle \mathsf{T}(x+y),x\rangle + \langle
\mathsf{T}(x+y),x \rangle\\
 &= \langle\mathsf{T}(x)+\mathsf{T}(y),x\rangle + \langle
 \mathsf{T}(x)+\mathsf{T}(y),y\rangle \\
 &= \langle \mathsf{T}(x),x \rangle + \langle \mathsf{T}(y),x \rangle +
 \langle \mathsf{T}(x),y\rangle + \langle \mathsf{T}(y),y\rangle\\
 &= \langle \mathsf{T}(y),x \rangle + \langle \mathsf{T}(x),y\rangle \\
 &= 0
 \end{align}
 \begin{equation}
 \implies \langle \mathsf{T}(y),x \rangle =  -\langle \mathsf{T}(x),y\rangle
 \end{equation}

 Let $
z = x + iy$
\begin{align}
\langle \mathsf{T}(z),z\rangle &= \langle \mathsf{T}(x+iy),x+iy\rangle
\\
&= \langle \mathsf{T}(x+iy),x\rangle + \langle
\mathsf{T}(x+iy),iy\rangle\\
&= \langle\mathsf{T}(x)+\mathsf{T}(iy),x\rangle + \langle
\mathsf{T}(x)+\mathsf{T}(iy),iy\rangle \\
&= \langle \mathsf{T}(x),x \rangle + \langle \mathsf{T}(iy),x \rangle +
\langle \mathsf{T}(x),iy\rangle + \langle \mathsf{T}(iy),iy\rangle\\
&= \langle \mathsf{T}(iy),x \rangle + \langle \mathsf{T}(x),iy\rangle
\\
&= i\langle\mathsf{T}(y),x \rangle + -i\langle\mathsf{T}(x),y\rangle\\
&= 0
\end{align}
\begin{equation}
\implies \langle\mathsf{T}(y),x \rangle = \langle\mathsf{T}(x),y\rangle
\end{equation}
\begin{gather}
\implies \langle\mathsf{T}(y),x \rangle =
\langle\mathsf{T}(x),y\rangle = - \langle\mathsf{T}(x),y\rangle\\
\implies \langle \mathsf{T}(y),x \rangle = \langle
\mathsf{T}(x),y\rangle =0 \quad \forall x,y \in \mathsf{V}
\end{gather}
Suppose $x,y$ are nonzero.
\begin{gather}
\langle \mathsf{T}(y),x\rangle = \langle 0,x\rangle = 0 \quad \forall
x \in \mathsf{V}\\
\implies \mathsf{T}(y) = 0 \quad \forall y \in \mathsf{V}\\
\implies \mathsf{T} = \mathsf{T}_0
\end{gather}
\item Suppose $\langle \mathsf{T}(x),x \rangle$ is real for all $x \in
  \mathsf{V}$

Claim: $\mathsf{T} = \mathsf{T}^*$

\begin{gather}
\langle \mathsf{T}(x),x \rangle = \overline{\langle
  \mathsf{T}(x),x\rangle}\quad \forall x \in \mathsf{V}\\
\overline{\langle \mathsf{T}(x),x \rangle} = \langle
x,\mathsf{T}(x)\rangle\\
\langle \mathsf{T}(x),x\rangle = \langle x,\mathsf{T}^*(x)\rangle\\
\implies \langle x, \mathsf{T}(x)\rangle = \langle x,\textsc{}
\mathsf{T}^*(x)\rangle \quad \forall x \in \mathsf{T}(x)\\
\implies \mathsf{T}(x) = \mathsf{T}^*(x) \quad \forall x \in
\mathsf{V}\\
\implies \mathsf{T} = \mathsf{T}^*
\end{gather}
\end{enumerate}
