Let $\mathsf{T}$ be a normal operator on a finite-dimensional inner
product space $\mathsf{V}.$ Prove that $N(\mathsf{T}) =
N(\mathsf{T}^*)$ and $R(\mathsf{T}) = R(\mathsf{T}^*).$

Claim:  $N(\mathsf{T}) = N(\mathsf{T}^*)$

$(\subseteq)$ Suppose $x \in N(\mathsf{T})$
\begin{gather}
\implies \mathsf{T}(x) = 0\cdot x\\
\implies \mathsf{T}^*(x) = \bar{0}\cdot x =0\quad\text{(Theorem 6.15.C)}\\ 
\implies x \in N(\mathsf{T}^*)
\end{gather}

$(\supseteq)$ Suppose $x \in N(\mathsf{T}^*)$
\begin{gather}
\implies \mathsf{T}^*(x) = 0 \cdot x\\
\implies \left(\mathsf{T}^*\right)^*(x) = \bar{0}\cdot x = x \quad\text{(Theorem 6.15.C)}\\
\left(\mathsf{T}^*\right)^*(x) = \mathsf{T}\\
\implies \mathsf{T}(x) = 0\\
\implies x \in N(\mathsf{T})
\end{gather}

Claim: $R(\mathsf{T}) = R(\mathsf{T}^*)$

\begin{gather}
N(\mathsf{T}) = N(\mathsf{T}^*)\\
N(\mathsf{T}^*) = R(\mathsf{T}^{**})^\perp = R(\mathsf{T})^\perp
\quad \text{(Problem 6.3.12)}\\
N(\mathsf{T}) = R(\mathsf{T}^*)^\perp \quad (\text{Problem 6.3.12})\\
\implies R(\mathsf{T}^*)^\perp = R(\mathsf{T})^\perp\\
\mathsf{V} =N(\mathsf{T})\oplus R(\mathsf{T}) = N(\mathsf{T}^*) \oplus R(\mathsf{T}^*)\\
\therefore \mathsf{V} = R(\mathsf{T}^*)^\perp \oplus R(\mathsf{T}^*) =
R(\mathsf{T})^\perp \oplus R(\mathsf{T})
\end{gather}
\newpage{}
$(\subseteq)$ Suppose $x \in R(\mathsf{T})$
\paragraph{Case 1} $x \neq 0$
\begin{gather}
\implies x \in R(\mathsf{T})^\perp \oplus R(\mathsf{T})\\
\implies x \in R(\mathsf{T}^*)^\perp \oplus R(\mathsf{T}^*)\\
\implies x \in R(\mathsf{T}^*)^\perp \text{ or } x \in
R(\mathsf{T}^*)\\
R(\mathsf{T}^*)^\perp = N(\mathsf{T}) \text{ and } x \notin N(\mathsf{T})\\
\implies x \in R(\mathsf{T}^*)
\end{gather}
\paragraph{Case 2} $x=0$
\begin{equation}
0 \in R(\mathsf{T^*})
\end{equation}

$(\supseteq)$ Suppose $x \in R(\mathsf{T}^*)$
\paragraph{Case 1} $x \neq 0$
\begin{gather}
\implies x \in R(\mathsf{T}^*)^\perp \oplus R(\mathsf{T}^*)\\
\implies x \in R(\mathsf{T})^\perp \oplus R(\mathsf{T})\\
\implies x \in R(\mathsf{T})^\perp \text{ or } x \in R(\mathsf{T})\\
R(\mathsf{T})^\perp = N(\mathsf{T}^*) \text{ and } x \notin
N(\mathsf{T}^*)\\
\implies x \in R(\mathsf{T})
\end{gather}
\paragraph{Case 2} $x = 0$
\begin{equation}
0 \in R(\mathsf{T})
\end{equation}
\begin{equation}
\therefore R(\mathsf{T}) = R(\mathsf{T}^*)
\end{equation}
