For each of the following matrices $A,$ find an orthogonal or unitary
matrix $P$ and a diagonal matrix $D$ such that $P^*AP = D.$ 
\begin{enumerate}
\item $\begin{pmatrix} 1 & 2 \\ 2 &1 \end{pmatrix}$
\begin{gather}
\det{
\begin{pmatrix}
1-\lambda & 2\\
2 & 1 -\lambda
\end{pmatrix}
}=(\lambda-3)(\lambda+1) = 0
\end{gather}
\begin{align}
\implies \lambda_1 &= -1\\
\lambda_2 &= 3
\end{align}
\begin{itemize}
\item For $\lambda_1 = -1$
\begin{gather}
\begin{pmatrix}
2 & 2\\
2 & 2
\end{pmatrix}
\begin{pmatrix}
x_1\\
x_2
\end{pmatrix}
=
\begin{pmatrix}
0\\
0
\end{pmatrix}\\
\implies x_1 = -x_2\\
\implies E_{\lambda_1} = \left\{
t\begin{pmatrix}-1\\1\end{pmatrix}\colon t\in \mathbb{R}
\right\}
\end{gather}
\item For $\lambda_2 = 3$
\begin{gather}
\begin{pmatrix}
-2 & 2 \\
2 & -2
\end{pmatrix}
\begin{pmatrix}
x_1\\
x_3
\end{pmatrix}
=
\begin{pmatrix}
0\\
0
\end{pmatrix}\\
\implies x_1 = x_2\\
\implies E_{\lambda_2} = \left\{
t\begin{pmatrix}1\\1\end{pmatrix} \colon t \in \mathbb{R}
\right\}
\end{gather}
\end{itemize}
Suppose
\begin{align}
w_1 = \begin{pmatrix}-1\\1\end{pmatrix} & & w_2 = \begin{pmatrix}1\\1\end{pmatrix}
\end{align}
Let
\begin{align}
v_1 &= w_1\\
v_2 &= w_2 - \frac{\langle w_2,v_1\rangle}{\norm{v_1}}v_1
\end{align}
\begin{gather}
\langle w_2,v_1 \rangle = 0\\
\implies v_2 = w_2\\
\norm{v_1}^2  = 2\\
\implies \norm{v_1} = \sqrt{2}\\
\implies o_1
= \begin{pmatrix}\frac{-1}{\sqrt{2}}\\\frac{1}{\sqrt{2}}\end{pmatrix}\\
\norm{v_2}^2 = 2\\
\implies \norm{v_2} = \sqrt{2}\\
\implies o_2 = \begin{pmatrix}\frac{1}{\sqrt{2}}\\\frac{-1}{\sqrt{2}}\end{pmatrix}
\end{gather}
Let 
\begin{gather}
P = \begin{pmatrix}
\frac{-1}{\sqrt{2}} & \frac{1}{\sqrt{2}}\\
\frac{1}{\sqrt{2}} & \frac{1}{\sqrt{2}}
\end{pmatrix}\\
P^t = \begin{pmatrix}
\frac{-1}{\sqrt{2}} & \frac{1}{\sqrt{2}}\\
\frac{1}{\sqrt{2}} & \frac{1}{\sqrt{2}}
\end{pmatrix}\\
P^tAP^t = D = \begin{pmatrix}
-1 & 0\\
0 & 3
\end{pmatrix}
\end{gather}
\item $\begin{pmatrix} 0 & -1\\1 & 0\end{pmatrix}$
\begin{gather}
\det{
\begin{pmatrix}
-\lambda & -1\\
1 & \lambda
\end{pmatrix}
} = 0\\
\lambda^2 +1 =0  
\end{gather}
\begin{align}
\implies \lambda_1 &= i\\
\lambda_2 &= -i
\end{align}
\begin{itemize}
\item For $\lambda_1 = i$
\begin{gather}
\begin{pmatrix}
-i & -1 \\
1 & -i
\end{pmatrix}
\begin{pmatrix}
x_1\\x_2
\end{pmatrix}
=
\begin{pmatrix}
0\\0
\end{pmatrix}\\
\begin{pmatrix}
-i & -1\\
i & 1
\end{pmatrix}
\begin{pmatrix}
x_1\\x_2
\end{pmatrix}
=
\begin{pmatrix}
0\\0
\end{pmatrix}\\
\implies x_1 = ix_2\\
\implies E_{\lambda_1} = \left\{
t\begin{pmatrix}i\\1\end{pmatrix}\colon t \in \mathbb{C}
\right\}
\end{gather}
\item For $\lambda_2 = -i$
\begin{gather}
\begin{pmatrix}
i & -1\\
1 & i
\end{pmatrix}
\begin{pmatrix}
x_1\\x_2
\end{pmatrix}
=
\begin{pmatrix}
0\\0
\end{pmatrix}\\
\begin{pmatrix}
0 & 0\\
i & -1
\end{pmatrix}
\begin{pmatrix}
x_1\\x_2
\end{pmatrix}
=
\begin{pmatrix}
0\\0
\end{pmatrix}\\
\implies x_1 = -ix_2\\
\implies E_{\lambda_2} =
\left\{t\begin{pmatrix}-i\\1\end{pmatrix}\colon t \in \mathbb{C}\right\}
\end{gather}
\end{itemize}
Suppose
\begin{align}
w_1 = \begin{pmatrix}i\\1\end{pmatrix} & & w_2 = \begin{pmatrix}-i\\1\end{pmatrix}
\end{align}
Let
\begin{align}
v_1 &= w_1\\
v_2 &= w_2 -\frac{\langle w_2,v_1\rangle}{\norm{v_1}}v_1
\end{align}
\begin{gather}
\langle w_2,v_1 \rangle = 0\\
\implies v_2 = w_2\\
\norm{v_1}^2 = 2\\
\implies \norm{v_1} = \sqrt{2}\\
\implies o_1
= \begin{pmatrix}\frac{i}{\sqrt{2}}\\\frac{1}{\sqrt{2}}\end{pmatrix}\\
\norm{v_2}^2 = 2\\
\implies \norm{v_2} = \sqrt{2}\\
\implies o_2 = \begin{pmatrix}\frac{-i}{\sqrt{2}}\\\frac{1}{\sqrt{2}}
\end{pmatrix}
\end{gather}
\begin{gather}
\implies P = \begin{pmatrix}
\frac{i}{\sqrt{2}} & \frac{-i}{\sqrt{2}}\\
\frac{1}{\sqrt{2}} & \frac{1}{\sqrt{2}}
\end{pmatrix}\\
\implies P^* = \begin{pmatrix}
\frac{-i}{\sqrt{2}} & \frac{1}{\sqrt{2}}\\
\frac{i}{\sqrt{2}} & \frac{1}{\sqrt{2}}
\end{pmatrix}\\
P^*AP = D = \begin{pmatrix}
i & 0\\
0 & -i
\end{pmatrix}
\end{gather}
\item $\begin{pmatrix}
2 & 3-3i\\
3+3i & 5
\end{pmatrix}$
\begin{gather}
\det{
\begin{pmatrix}
2-\lambda & 3-3i\\
3+3i & 5-\lambda
\end{pmatrix}
}=0\\
(\lambda -8)(\lambda+1) = 0
\end{gather}
\begin{align}
\implies \lambda_1 = -1\\
\lambda_2 = 8
\end{align}
\begin{itemize}
\item For $\lambda_1 = -1$
\begin{gather}
\begin{pmatrix}
3 & 3-3i\\
3+3i & 6
\end{pmatrix}
\begin{pmatrix}
x_1 \\x_2
\end{pmatrix}
\begin{pmatrix}
0\\0
\end{pmatrix}\\
\begin{pmatrix}
1 & 1-i\\
1+i & 2
\end{pmatrix}
\begin{pmatrix}
x_1 \\x_2
\end{pmatrix}
\begin{pmatrix}
0\\0
\end{pmatrix}\\
\implies x_1 = x_2(i-1)\\
\implies E_{\lambda_1} = \left\{
t\begin{pmatrix}-1 +i\\1\end{pmatrix}\colon t \in \mathbb{C}
\right\}
\end{gather}
\item For $\lambda_2 = 8$
\begin{gather}
\begin{pmatrix}
-6 & 3-3i\\
3+3i & -3
\end{pmatrix}
\begin{pmatrix}
x_1 \\x_2
\end{pmatrix}
\begin{pmatrix}
0\\0
\end{pmatrix}\\
\begin{pmatrix}
0 & 0\\
2 & i-1
\end{pmatrix}
\begin{pmatrix}
x_1 \\x_2
\end{pmatrix}
\begin{pmatrix}
0\\0
\end{pmatrix}\\
\implies x_1 = \frac{1-i}{2}x_2\\
\implies E_{\lambda_2} = \left\{
t\begin{pmatrix}\frac{1-i}{2}\\1\end{pmatrix}\colon t \in \mathbb{C}
\right\}
\end{gather}
\end{itemize}
Suppose
\begin{align}
w_1 = \begin{pmatrix}-1 + i\\1\end{pmatrix} & & w_2 = \begin{pmatrix}\frac{1-i}{2}\\1\end{pmatrix}
\end{align}
Let
\begin{align}
v_1 &= w_1\\
v_2 &= w_2 - \frac{\langle w_2,v_1\rangle}{\norm{v_1}}v_1
\end{align}
\begin{gather}
\langle w_2,v_1 \rangle = 0 \\
\implies v_2 = w_2\\
\norm{v_1}^2 = 3\\
\implies \norm{v_1} = \sqrt{3}\\
\implies o_1 = \begin{pmatrix}
\frac{-1+i}{\sqrt{3}}\\\frac{1}{\sqrt{3}}
\end{pmatrix}\\
\norm{v_2}^2 = \frac{3}{2}\\
\norm{v_2} = \sqrt{\frac{3}{2}}\\
\implies o_2  = \begin{pmatrix}
\frac{1-i}{\sqrt{6}}\\\sqrt{\frac{2}{3}}
\end{pmatrix}
\end{gather}
\begin{gather}
\implies P = \begin{pmatrix}
\frac{-i+1}{\sqrt{3}} & \frac{1-i}{\sqrt{6}}\\
\frac{1}{\sqrt{2}}  & \sqrt{\frac{2}{3}}
\end{pmatrix}\\
\implies P^* = \begin{pmatrix}
\frac{-i-i}{\sqrt{3}} & \frac{1}{\sqrt{2}}\\
\frac{1+i}{\sqrt{6}} & \sqrt{\frac{2}{3}}
\end{pmatrix}\\
\implies P^*AP = D = \begin{pmatrix}
-1 & 0\\
0 & 8
\end{pmatrix}
\end{gather}
\item $\begin{pmatrix}
0 & 2 & 2\\
2 & 0 & 2\\
2 & 2 & 0
\end{pmatrix}$
\begin{gather}
\det{
\begin{pmatrix}
-\lambda & 2 & 2\\
2 & -\lambda & 2\\
2 & 2 & -\lambda
\end{pmatrix}
}=0\\
\implies (z+2)^2(x-4) = 0
\end{gather}
\begin{align}
\implies \lambda_1 &= -2\\
\lambda_2 &= 4
\end{align}
\begin{itemize}
\item For $\lambda_1 = -2$
\begin{gather}
\begin{pmatrix}
-2 & 2 & 2\\
2 & -2 & 2\\
2 & 2 & -2
\end{pmatrix}
\begin{pmatrix}
x_1\\x_2\\x_3
\end{pmatrix}
=
\begin{pmatrix}
0\\0\\0
\end{pmatrix}\\
\begin{pmatrix}
1 & 1 & 1\\
0 & 0 & 0\\
0 & 0 & 0
\end{pmatrix}
\begin{pmatrix}
x_1\\x_2\\x_3
\end{pmatrix}
=
\begin{pmatrix}
0\\0\\0
\end{pmatrix}\\
\implies x_1 = -x_2 + -x_3\\
\implies E_{\lambda_1} = \left\{
t\begin{pmatrix}-1\\1\\0\end{pmatrix}
+s\begin{pmatrix}-1\\0\\1\end{pmatrix}\colon t,s \in \mathbb{R}
\right\}
\end{gather}
\item For $\lambda_2 = 4$
\begin{gather}
\begin{pmatrix}
-4 & 2 & 2\\
2 & -4 & 2\\
2 & 2 & -4
\end{pmatrix}
\begin{pmatrix}
x_1\\x_2\\x_3
\end{pmatrix}
=
\begin{pmatrix}
0\\0\\0
\end{pmatrix}\\
\begin{pmatrix}
0 & 1 & -1\\
1 & 0 & -1\\
0 & 0 & 0
\end{pmatrix}
\begin{pmatrix}
x_1\\x_2\\x_3
\end{pmatrix}
=
\begin{pmatrix}
0\\0\\0
\end{pmatrix}\\
\implies x_1 = x_3\\
x_2 = x_3\\
\implies E_{\lambda_2} = \left\{
t\begin{pmatrix}1\\1\\1\end{pmatrix}\colon t \in \mathbb{R}
\right\}
\end{gather}
\end{itemize}
Suppose
\begin{align}
w_1 = \begin{pmatrix}-1\\1\\0\end{pmatrix} & & w_2
= \begin{pmatrix}-1\\0\\1\end{pmatrix} & & w_3 =\begin{pmatrix}1\\1\\1\end{pmatrix}
\end{align}
Let
\begin{align}
v_1 &= w_1\\
v_2 &= w_2 - \frac{\langle w_2,v_2\rangle}{\norm{v_1}^2}v_1\\
v_3 &= w_3 - \left(\frac{\langle w_3,v_2\rangle}{\norm{v_2}^2}v_2 +
  \frac{\langle w_3,v_1\rangle}{\norm{v_1}^2}v_1\right)\\
\end{align}
\begin{gather}
\langle w_2,v_1 \rangle = 1\\
\norm{v_1}^2 = 2\\
\implies \norm{v_1} = \sqrt{2}\\
\implies o_1 = \begin{pmatrix}\frac{-1}{\sqrt{2}}\\\frac{1}{\sqrt{2}}\\0\end{pmatrix}\\
\implies v_2
= \begin{pmatrix}\mfrac{-1}{2}\\\mfrac{-1}{2}\\1\end{pmatrix}\\
\norm{v_2}^2 = 2\\
\implies \norm{v_2} = \sqrt{2}\\
\implies o_2 = \begin{pmatrix}\frac{-1}{\sqrt{2}}\\0\\\frac{1}{\sqrt{2}}\end{pmatrix}\\
\langle w_3,v_2\rangle = 0\\
\langle w_3,v_2 \rangle = 0\\
\implies v_3 = w_3\\
\norm{v_3}^2 = 3\\
\implies \norm{v_3} = \sqrt{3}\\
\implies o_3 = \begin{pmatrix}\frac{1}{\sqrt{3}}\\\frac{1}{\sqrt{3}}\\\frac{1}{\sqrt{3}}\end{pmatrix}
\end{gather}
\begin{gather}
\implies P = \begin{pmatrix}
\frac{-1}{\sqrt{2}} & \frac{-1}{\sqrt{2}} & \frac{1}{\sqrt{3}}\\
\frac{1}{\sqrt{2}} & 0 & \frac{1}{\sqrt{3}}\\
0 & \frac{1}{\sqrt{2}} & \frac{1}{\sqrt{3}}
\end{pmatrix}\\
\implies P^* = \begin{pmatrix}
\frac{-1}{\sqrt{2}} & \frac{1}{\sqrt{2}} & 0\\
\frac{-1}{\sqrt{2}} & 0 & \frac{1}{\sqrt{2}}\\
\frac{1}{\sqrt{3}} & \frac{1}{\sqrt{3}} & \frac{1}{\sqrt{3}}
\end{pmatrix}\\
P^*AP = D = \begin{pmatrix}
-2 & 0 & 0\\
0 & -2 & 0\\
0 & 0 & 4
\end{pmatrix}
\end{gather}
\item $\begin{pmatrix}
2 & 1 & 1 \\
1 & 2 & 1\\
1 & 1 & 2
  \end{pmatrix}$
\begin{gather}
\det{
\begin{pmatrix}
2-\lambda & 1 & 1 \\
1 & 2-\lambda & 1\\
1 & 1 & 2-\lambda
\end{pmatrix}
}=0\\
(1-\lambda)^2(\lambda-4)
\end{gather}
\begin{align}
\implies \lambda_1 &= 1\\
\lambda_2 &= 4
\end{align}
\begin{itemize}
\item For $\lambda_1=1$
\begin{gather}
\begin{pmatrix}
1 & 1 & 1\\
1 & 1 & 1\\
1 & 1 & 1
\end{pmatrix}
\begin{pmatrix}
x_1\\x_2\\x_3
\end{pmatrix}
=
\begin{pmatrix}
0\\0\\0
\end{pmatrix}\\
\begin{pmatrix}
1 & 1 & 1\\
0 & 0 & 0\\
0 & 0 & 0
\end{pmatrix}
\begin{pmatrix}
x_1\\x_2\\x_3
\end{pmatrix}
=
\begin{pmatrix}
0\\0\\0
\end{pmatrix}\\
\implies x_1 = -x_2+-x_3\\
\implies E_{\lambda_1} = \left\{
t\begin{pmatrix}-1\\1\\0\end{pmatrix}\colon t,s \in \mathbb{R}
\right\}
\end{gather}
\item For $\lambda_2 = 4$
\begin{gather}
\begin{pmatrix}
-2 & 1 & 1\\
1 & -2 & 1\\
1 & 1 & -2
\end{pmatrix}
\begin{pmatrix}
x_1\\x_2\\x_3
\end{pmatrix}
=
\begin{pmatrix}
0\\0\\0
\end{pmatrix}\\
\implies E_{\lambda_2} = \left\{
t\begin{pmatrix}1\\1\\1\end{pmatrix}\colon t \in \mathbb{R}
\right\}
\end{gather}
\end{itemize}
Suppose
\begin{align}
w_1 = \begin{pmatrix}-1\\1\\0\end{pmatrix} & & w_2
= \begin{pmatrix}-1\\0\\1\end{pmatrix} & & w_3 =\begin{pmatrix}1\\1\\1\end{pmatrix}
\end{align}
Let
\begin{align}
v_1 &= w_1\\
v_2 &= w_2 - \frac{\langle w_2,v_2\rangle}{\norm{v_1}^2}v_1\\
v_3 &= w_3 - \left(\frac{\langle w_3,v_2\rangle}{\norm{v_2}^2}v_2 +
  \frac{\langle w_3,v_1\rangle}{\norm{v_1}^2}v_1\right)\\
\end{align}
\begin{gather}
\langle w_2,v_1 \rangle = 1\\
\norm{v_1}^2 = 2\\
\implies \norm{v_1} = \sqrt{2}\\
\implies o_1 = \begin{pmatrix}\frac{-1}{\sqrt{2}}\\\frac{1}{\sqrt{2}}\\0\end{pmatrix}\\
\implies v_2
= \begin{pmatrix}\mfrac{-1}{2}\\\mfrac{-1}{2}\\1\end{pmatrix}\\
\norm{v_2}^2 = 2\\
\implies \norm{v_2} = \sqrt{2}\\
\implies o_2 = \begin{pmatrix}\frac{-1}{\sqrt{2}}\\0\\\frac{1}{\sqrt{2}}\end{pmatrix}\\
\langle w_3,v_2\rangle = 0\\
\langle w_3,v_2 \rangle = 0\\
\implies v_3 = w_3\\
\norm{v_3}^2 = 3\\
\implies \norm{v_3} = \sqrt{3}\\
\implies o_3 = \begin{pmatrix}\frac{1}{\sqrt{3}}\\\frac{1}{\sqrt{3}}\\\frac{1}{\sqrt{3}}\end{pmatrix}
\end{gather}
\begin{gather}
\implies P = \begin{pmatrix}
\frac{-1}{\sqrt{2}} & \frac{-1}{\sqrt{2}} & \frac{1}{\sqrt{3}}\\
\frac{1}{\sqrt{2}} & 0 & \frac{1}{\sqrt{3}}\\
0 & \frac{1}{\sqrt{2}} & \frac{1}{\sqrt{3}}
\end{pmatrix}\\
\implies P^* = \begin{pmatrix}
\frac{-1}{\sqrt{2}} & \frac{1}{\sqrt{2}} & 0\\
\frac{-1}{\sqrt{2}} & 0 & \frac{1}{\sqrt{2}}\\
\frac{1}{\sqrt{3}} & \frac{1}{\sqrt{3}} & \frac{1}{\sqrt{3}}
\end{pmatrix}\\
P^*AP = D = \begin{pmatrix}
1 & 0 & 0 \\
0 & 1 & 0\\
0 & 0 & 4
\end{pmatrix}
\end{gather}
\end{enumerate}
